theories/TensorAutomation/TensorExprDBSyntax.v
@@ -4,93 +4,10 @@ Require StringCustomNotation.
 From stdpp Require Import strings fin_maps pmap gmap.
 From stdpp Require Import pretty.
 
-Require Import Aux_stdpp.
-
-Definition pos_to_nat_pred (p : positive) : nat :=
-  pred (Pos.to_nat p).
+Require Import Aux_stdpp Aux_pos.
 
 #[local] Coercion pos_to_nat_pred : positive >-> nat.
-
-Definition pos_add_N (p : positive) (n : N) : positive :=
-  match n with
-  | N0 => p
-  | Npos q => Pos.add p q
-  end.
-
-Lemma pos_add_N_to_Z n p : (Zpos (pos_add_N p n) = Zpos p + Z.of_N n)%Z.
-Proof.
-  unfold pos_add_N; destruct n; lia.
-Qed.
-
-
-Definition pos_sub_N (p : positive) (n : N) : positive :=
-  match n with
-  | N0 => p
-  | Npos q => Pos.sub p q
-  end.
-
-Lemma pos_sub_N_to_Z n p : N.lt n (Npos p) ->
-  (Zpos (pos_sub_N p n) = Zpos p - Z.of_N n)%Z.
-Proof.
-  unfold pos_sub_N; destruct n; lia.
-Qed.
-
-(* FIXME: Move *)
-#[global]
-Program Instance Op_pos_to_nat_pred : ZifyClasses.UnOp pos_to_nat_pred :=
-  { TUOp x := (x - 1)%Z }.
-Next Obligation.
-  cbn.
-  unfold pos_to_nat_pred.
-  intros; lia.
-Qed.
-Add Zify UnOp Op_pos_to_nat_pred.
-
-#[global]
-Program Instance Op_pos_add_N : ZifyClasses.BinOp pos_add_N :=
-  { TBOp x y := (x + y)%Z }.
-Next Obligation.
-  cbn.
-  intros.
-  apply pos_add_N_to_Z.
-Qed.
-Add Zify BinOp Op_pos_add_N.
-
-#[global]
-Program Instance Op_pos_sub_N : ZifyClasses.BinOp pos_sub_N :=
-  { TBOp x y := Z.max 1 (x - y)%Z }.
-Next Obligation.
-  cbn.
-  intros.
-  unfold pos_sub_N.
-  destruct m; lia.
-Qed.
-Add Zify BinOp Op_pos_sub_N.
-
-
-(* FIXME: Move *)
-Section lengthN.
-
-Local Open Scope N_scope.
-
-Fixpoint lengthN {A} (l : list A) : N :=
-  match l with
-  | [] => 0%N
-  | _ :: l => N.succ (lengthN l)
-  end.
-Lemma lengthN_correct {A} (l : list A) :
-  N.to_nat (lengthN l) = length l.
-Proof. induction l; cbn; lia. Qed.
-Lemma lengthN_correct_rev {A} (l : list A) :
-  lengthN l = N.of_nat (length l).
-Proof. rewrite <- lengthN_correct; lia. Qed.
-Lemma lengthN_app {A} (l l' : list A) :
-  lengthN (l ++ l') = lengthN l + lengthN l'.
-Proof.
-  now rewrite 3 lengthN_correct_rev, length_app, Nat2N.inj_add.
-Qed.
-
-End lengthN.
+#[local] Coercion N.of_nat : nat >-> N.
 
 
 (* Section TensorExprDB.  *)
@@ -199,6 +116,13 @@ Proof.
   intros fr fr' Hfr fl fl' Hfl fg fg' Hfg [];
   cbn; f_equal; auto.
 Qed.
+
+Definition var_elim {A : Type} (fr fl fg : Idx -> A) : var -> A :=
+  fun v => match v with
+  | rel r => fr r
+  | loc l => fl l
+  | glob g => fg g
+  end.
 
 
 Inductive tensorexpr :=
@@ -496,10 +420,9 @@ Definition abstracts_global_vars
 
 
 
-
 (** Relabeling in [tensorlist]s *)
 
-Definition relabel_abs (f : var -> var) (abs : Idx * list var * list var) :=
+Definition relabel_abs {A B} (f : B -> A) (abs : Idx * list B * list B) :=
   let '(idx, lower, upper) := abs in
   (idx, f <$> lower, f <$> upper).
 
@@ -545,50 +468,22 @@ Definition tl_times (l r : tensorlist) : tensorlist :=
   mk_tl (lsums ++ rsums) (labs' ++ rabs').
 
 
-(* FIXME: Move *)
-Lemma list_fmap_id' `(f : A -> A) (l : list A) :
-  (forall a, a ∈ l -> f a = a) ->
-  f <$> l = l.
-Proof.
-  intros Hf.
-  etransitivity; [|apply list_fmap_id].
-  apply list_fmap_ext; intros _ ? ?%elem_of_list_lookup_2.
-  now apply Hf.
-Qed.
-
-Ltac tspecialize_with C tac :=
-  match type of C with
-  | forall _ : ?A, _ =>
-    let H := fresh in
-    assert (H : A); [
-      tac | specialize (C H); clear H
-    ]
-  end.
-
-Tactic Notation "tspecialize" uconstr(C) "by" tactic3(tac) :=
-  tspecialize_with C ltac:(solve [tac]).
-
-Tactic Notation "tspecialize" uconstr(C) :=
-  tspecialize_with C ltac:(idtac).
-
-#[local] Coercion N.of_nat : nat >-> N.
-
-Lemma relabel_abs_id abs : relabel_abs id abs = abs.
+Lemma relabel_abs_id {A} abs : relabel_abs (@id A) abs = abs.
 Proof.
   destruct abs as [[f low] up]; cbn.
   now rewrite 2 list_fmap_id.
 Qed.
 
-Lemma relabel_abs_ext f g abs :
-  (forall x, f x = g x) -> relabel_abs f abs = relabel_abs g abs.
+Lemma relabel_abs_ext {A B} f g abs :
+  (forall x, f x = g x) -> @relabel_abs A B f abs = relabel_abs g abs.
 Proof.
   intros Heq.
   destruct abs as [[idx low] up]; cbn.
   f_equal; [f_equal|]; apply list_fmap_ext; intros; apply Heq.
 Qed.
 
-Lemma relabel_abs_id' f abs :
-  (forall x, f x = x) -> relabel_abs f abs = abs.
+Lemma relabel_abs_id' {A} f abs :
+  (forall x : A, f x = x) -> relabel_abs f abs = abs.
 Proof.
   intros Hid.
   erewrite relabel_abs_ext; [apply relabel_abs_id|apply Hid].
@@ -658,20 +553,20 @@ Fixpoint tensorlist_of_tensorexpr (te : tensorexpr) : tensorlist :=
 
 (* TO DO: When I figure out the "boundary condition" or whatever that is,
    incorporate it into the function at this level somehow? *)
-(* TODO: Figure out incorporating typing into this!! As-is this will be 
+(* TODO: Figure out incorporating typing into this!! As-is this will be
   hard to reason about without WF conditions*)
-  (* TODO: Why do I hate WF conditions? TODO: Do I hate WF conditions? 
+  (* TODO: Why do I hate WF conditions? TODO: Do I hate WF conditions?
     Checking it is probably a pretty small price to pay... especially at
     the tensorlist level*)
 Fixpoint extend_map_of_abstract_pair
-  (mb mbi : Pmap Idx) (* The map and inverse map of [rel]/bound variables, 
+  (mb mbi : Pmap Idx) (* The map and inverse map of [rel]/bound variables,
     which must map to other bound variables *)
   (ml : Pmap var) (* The map of local variables, which can map to any [var] *)
   (mlran : Pset) (* The set of [rel] variables in the range of [ml], which
      must be disjoint from the image of [mb] / domain of [mbi] *)
-  (l r : list var) : option (Pmap Idx * Pmap Idx * Pmap var) :=
+  (l r : list var) : option (Pmap Idx * Pmap Idx * Pmap var * Pset) :=
   match l, r with
-  | [], [] => Some (mb, mbi, ml)
+  | [], [] => Some (mb, mbi, ml, mlran)
   | hl :: l, hr :: r =>
     match hl, hr with
     | glob gl, glob gr => (* global variables must match exactly! *)
@@ -682,16 +577,16 @@ Fixpoint extend_map_of_abstract_pair
       None
     | loc ll, vr => (* local variables can map anywhere (ab initio, at least) *)
       match ml !! ll with
-      | None => 
-        match vr with 
-        | rel rr => 
+      | None =>
+        match vr with
+        | rel rr =>
           match mbi !! rr with
           | Some _ => None (* This variable is already bound; we can't use it locally *)
           | None =>
-            extend_map_of_abstract_pair mb mbi (<[ll := rel rr]> ml) ({[rr]} ∪ mlran) 
+            extend_map_of_abstract_pair mb mbi (<[ll := rel rr]> ml) ({[rr]} ∪ mlran)
               l r
           end
-        | vr => 
+        | vr =>
           extend_map_of_abstract_pair mb mbi (<[ll := vr]> ml) mlran l r
         end
       | Some vr' =>
@@ -701,14 +596,14 @@ Fixpoint extend_map_of_abstract_pair
       end
     | rel rl, rel rr => (* bound variables must map to bound variables *)
       match mb !! rl with
-      | None => 
+      | None =>
         match mbi !! rr with (* Preserve the inverses! *)
-        | None => 
-          if bool_decide (rr ∈ mlran) then 
+        | None =>
+          if bool_decide (rr ∈ mlran) then
             (* This relative variable is mapped to by a local variable already *)
-            None 
-          else 
-            extend_map_of_abstract_pair 
+            None
+          else
+            extend_map_of_abstract_pair
               (<[rl := rr]> mb) (<[rr := rl]> mbi) ml mlran l r
         | Some _ => None (* This variable is already mapped to *)
         end
@@ -739,10 +634,10 @@ Definition list_first_omap {A B} (f : A -> option B) : list A -> option B :=
 (* TODO: rewrite with collate (also, optionally shortcut to false if
   we don't use up all the abstracts for a given index) *)
 Fixpoint extend_match_of_abstract_tensors
-  (P : Pmap Idx -> Pmap Idx -> Pmap var -> Pset -> 
+  (P : Pmap Idx -> Pmap Idx -> Pmap var -> Pset ->
     list (Idx * list var * list var) -> Prop)
   `{HP : forall mb mbi ml mlran rrest, Decision (P mb mbi ml mlran rrest)}
-  (mb mbi : Pmap Idx) (* The map and inverse map of [rel]/bound variables, 
+  (mb mbi : Pmap Idx) (* The map and inverse map of [rel]/bound variables,
     which must map to other bound variables *)
   (ml : Pmap var) (* The map of local variables, which can map to any [var] *)
   (mlran : Pset) (* The set of [rel] variables in the range of [ml], which
@@ -756,8 +651,8 @@ Fixpoint extend_match_of_abstract_tensors
     else None
   | (fl, lowl, upl) :: labs =>
     list_first_omap (fun '((_, lowr, upr), rrest) =>
-      '(mb, mbi, ml) ← extend_map_of_abstract_pair mb mbi ml mlran lowl lowr;
-         '(mb, mbi, ml) ← extend_map_of_abstract_pair mb mbi ml mlran upl upr;
+      '(mb, mbi, ml, mlran) ← extend_map_of_abstract_pair mb mbi ml mlran lowl lowr;
+         '(mb, mbi, ml, mlran) ← extend_map_of_abstract_pair mb mbi ml mlran upl upr;
         extend_match_of_abstract_tensors P mb mbi ml mlran labs rrest)
       (list_select (fun '(fr, _, _) => fl = fr) rabs)
     (* head ('((_, lowr, upr), rrest) ← list_select (fun '(fr, _, _) => fl = fr) rabs;
@@ -768,7 +663,7 @@ Fixpoint extend_match_of_abstract_tensors
       ) *)
   end.
 
-(* TODO: Theory of: 
+(* TODO: Theory of:
 Definition lookup _ endomorphism `{Lookup A A M} (m : M) : A -> A :=
   fun a => default a (m !! a). *)
 
@@ -776,74 +671,85 @@ Definition lookup _ endomorphism `{Lookup A A M} (m : M) : A -> A :=
 Definition Pmap_map (m : Pmap Idx) : Idx -> Idx :=
   fun v => default v (m !! v).
 
-Definition match_tensorlist_aux (tl tl' : tensorlist) : 
+Definition match_tensorlist_aux (tl tl' : tensorlist) :
   option (tensorlist * (* What remains of [tl'] after the match of [tl] is removed *)
   Pmap Idx * (* The mapping of _unmatched_ bound variables from the unmatched
     portion of [tl'] to those in the returned tensorlist *)
   Pmap var) (* The mapping of the local variables of [tl] to variables of
     [tl'], possibly including relative variables (which are reindexed to
-      be correct within the returned tensorlist; however, they must be 
+      be correct within the returned tensorlist; however, they must be
       shifted along with the variables of the abstracts of the returned
       tensorlist if (innermost) sums are added to the tensorlist) *) :=
   match extend_match_of_abstract_tensors
-    (fun mb mbi ml mlran rabs => 
+    (fun mb mbi ml mlran rabs =>
       (* TODO: Check this progressively, using [collate] *)
       set_Forall (λ r, ~ is_Some (mbi !! r)) (abstracts_rel_vars rabs))
-    ∅ ∅ ∅ ∅ (tl.(tl_abstracts)) (tl'.(tl_abstracts)) with 
+    ∅ ∅ ∅ ∅ (tl.(tl_abstracts)) (tl'.(tl_abstracts)) with
   | None => None
   | Some (mb, mbi, ml, mlran, rrest) =>
-  
-  (* We have: [mb/mbi] : maps [Idx -> Idx] such that 
+
+  (* We have: [mb/mbi] : maps [Idx -> Idx] such that
     [mb <$> tl] is a subexpression of [tl']; notably:
-    (i) the sums not included in [mb <$> tl] are those of [tl'] 
+    (i) the sums not included in [mb <$> tl] are those of [tl']
       that are _not_ included in [img mb = dom mbi]
-    (ii) the abstracts not included in [mb <$> tl] are [rrest] 
-    
+    (ii) the abstracts not included in [mb <$> tl] are [rrest]
+
     We need two maps [reord reord_rest : Idx -> Idx] such that
     [reord_rest <$> rrest] makes the variables correct there, assuming
-    we simply remove the match (we also need to figure out the order of 
+    we simply remove the match (we also need to figure out the order of
     types; same thing), and such that [reord]
     *)
   Some (
-  let ntys := imap (fun i ty => (Pos.of_succ_nat i, ty)) (reverse tl'.(tl_sums)) in 
-  let unused_tys := filter (fun '(idx, _) => ~ is_Some (mbi !! idx)) ntys in 
-  let newty_info := imap (fun inew '(iold, ty) => (iold, Pos.of_succ_nat inew, ty)) unused_tys in 
-  let rrest_map : Pmap _ := list_to_map newty_info.*1 in 
-  let newtys := reverse newty_info.*2 in 
+  let ntys := imap (fun i ty => (Pos.of_succ_nat i, ty)) (reverse tl'.(tl_sums)) in
+  let unused_tys := filter (fun '(idx, _) => ~ is_Some (mbi !! idx)) ntys in
+  let newty_info := imap (fun inew '(iold, ty) => (iold, Pos.of_succ_nat inew, ty)) unused_tys in
+  let rrest_map : Pmap _ := list_to_map newty_info.*1 in
+  let newtys := reverse newty_info.*2 in
   let ml' := (relabel_rels (Pmap_map rrest_map) <$> ml) in
-  (mk_tl newtys (relabel_abs (relabel_rels (Pmap_map rrest_map)) <$> 
+  (mk_tl newtys (relabel_abs (relabel_rels (Pmap_map rrest_map)) <$>
     rrest),
   rrest_map, ml'))
   end.
 
 Definition var_subst_locals (f : Idx -> var) (v : var) : var :=
-  match v with 
+  match v with
   | loc l => f l
   | _ => v
   end.
 
-(* TODO: Definitely need to make sure [ml] maps locals to variables 
-  of the correct type. Can do this with overall WF of goal (can get 
+(* TODO: Definitely need to make sure [ml] maps locals to variables
+  of the correct type. Can do this with overall WF of goal (can get
   all typing from the abstract map, then check; if [lhs == rhs] not
   WF, we should still maybe be fine? I'd thought this worked before
   but now I'm not positive). *)
 
 (* Assuming [lhs == rhs] (for the moment, ignore typing and context),
   rewrite this equality in [targ], if possible. *)
-Definition match_rewrite_tensorlist (lhs rhs targ : tensorlist) : 
-  option tensorlist := 
+Definition match_rewrite_tensorlist (lhs rhs targ : tensorlist) :
+  option tensorlist :=
   '((mk_tl usums uabs), relmap, locmap) ← match_tensorlist_aux lhs targ;
-  let '(mk_tl rsums rabs) := rhs in 
-  let rsize := lengthN rsums in 
-  let shift := relabel_rels (λ p, pos_add_N p rsize) in 
-  let uabs_shifted := relabel_abs shift <$> uabs in 
-  let rabs_subst := relabel_abs (var_subst_locals (λ l, 
-    from_option shift (loc l) (locmap !! l))) <$> rabs in 
+  let '(mk_tl rsums rabs) := rhs in
+  let rsize := lengthN rsums in
+  let shift := relabel_rels (λ p, pos_add_N p rsize) in
+  let uabs_shifted := relabel_abs shift <$> uabs in
+  let rabs_subst := relabel_abs (var_subst_locals (λ l,
+    from_option shift (loc l) (locmap !! l))) <$> rabs in
   Some (mk_tl (usums ++ rsums) (uabs_shifted ++ rabs_subst)).
 
+Definition fill_tensorlist_rewrite (outer : tensorlist) (inner : tensorlist)
+  (relmap : Pmap Idx) (locmap : Pmap var) : tensorlist :=
+  let '(mk_tl usums uabs) := outer in (* 'unmatched' sums and abtracts *)
+  let '(mk_tl rsums rabs) := inner in (* the 'right-hand side' *)
+  let rsize := lengthN rsums in
+  let shift := relabel_rels (λ p, pos_add_N p rsize) in
+  let uabs_shifted := relabel_abs shift <$> uabs in
+  let rabs_subst := relabel_abs (var_subst_locals (λ l,
+    from_option shift (loc l) (locmap !! l))) <$> rabs in
+  mk_tl (usums ++ rsums) (uabs_shifted ++ rabs_subst).
 
 
-(* 
+
+(*
 
 Record namedtensorlist := mk_ntl {
   ntl_sums : list (Idx * Ty);
@@ -852,15 +758,15 @@ Record namedtensorlist := mk_ntl {
 
 
 Definition ntl2tl (ntl : namedtensorlist) :=
-  let '(mk_ntl sums abs) := ntl in 
-  let varmap : Pmap Idx := list_to_map 
+  let '(mk_ntl sums abs) := ntl in
+  let varmap : Pmap Idx := list_to_map
     (imap (λ idx '(r, ty), (r, Pos.of_succ_nat idx))
       sums) in
   mk_tl sums.*2
   (relabel_abs (relabel_rels (λ v, default v (varmap !! v))) <$> abs).
 
-Definition tl2ntl (tl : tensorlist) := 
-  let '(mk_tl sums abs) := tl in 
+Definition tl2ntl (tl : tensorlist) :=
+  let '(mk_tl sums abs) := tl in
   mk_ntl (imap (λ i v, (Pos.of_succ_nat i, v)) (reverse sums))
     abs.
 
@@ -878,26 +784,26 @@ Definition WF_tl (tl : tensorlist) : Prop :=
     (fun mb mbi ml mlran rabs => rabs = [])
     ∅ ∅ ∅ ∅ (tl.(tl_abstracts)) (tl'.(tl_abstracts)). *)
 
-Definition make_match_namedtensorlist_data 
-  (rsums : list (Idx * Ty)) (rabs : list _) 
+Definition make_match_namedtensorlist_data
+  (rsums : list (Idx * Ty)) (rabs : list _)
   (mbi : Pmap Idx) : namedtensorlist :=
   mk_ntl (filter (λ '(idx, ty), ~ is_Some (mbi !! idx)) rsums) rabs.
 
 Definition match_namedtensorlist_aux (tl tl' : namedtensorlist) :
   option (namedtensorlist * Pmap Idx * Pmap Idx * Pmap var * Pset) :=
   '(mb, mbi, ml, mlran, rrest) ← extend_match_of_abstract_tensors
-    (fun mb mbi ml mlran rabs => 
+    (fun mb mbi ml mlran rabs =>
       set_Forall (λ r, ~ is_Some (mbi !! r)) (abstracts_rel_vars rabs))
     ∅ ∅ ∅ ∅ (tl.(ntl_abstracts)) (tl'.(ntl_abstracts));
-  Some (make_match_namedtensorlist_data tl'.(ntl_sums) rrest mbi, 
+  Some (make_match_namedtensorlist_data tl'.(ntl_sums) rrest mbi,
     mb, mbi, ml, mlran).
 
-Definition match_rewrite_namedtensorlist (lhs rhs target : namedtensorlist) : 
+Definition match_rewrite_namedtensorlist (lhs rhs target : namedtensorlist) :
   option namedtensorlist :=
-  '() match_namedtensorlist_aux lhs target with 
+  '() match_namedtensorlist_aux lhs target with
   | None => None
   | (* TODO: Problem!!! Here, I want to insert the rhs—but the bound variables
-    could conflict! I want to work only with WF namedtensorlist, so this is 
+    could conflict! I want to work only with WF namedtensorlist, so this is
     actually a big problem. (Un)Fortunately, there's a simple solution: I just
     need to work with [tensorlist]s exclusively (yes, with all the relabeling
     hell that will create). I believe the algorithm should be essentially the
@@ -908,7 +814,7 @@ Definition match_tensorlist *)
 
 
 
-(* OLD: 
+(* OLD:
 
 (* Matching on [tensorlist]s *)
 
@@ -1000,5 +906,2434 @@ Definition match_tensorlist (tl tl' : tensorlist) :
 
 
 *)
+
+
+
+
+
+
+
+
+
+Record tensorequation := mk_teq {
+  teq_lhs : tensorexpr;
+  teq_rhs : tensorexpr;
+  teq_univ : Pmap Ty;
+    (* The set of universally-quantified variables and their types *)
+}.
+
+
+Record tensorlistequation := mk_tleq {
+  tleq_lhs : tensorlist;
+  tleq_rhs : tensorlist;
+  tleq_univ : Pmap Ty;
+    (* The set of universally-quantified variables and their types *)
+}.
+
+
+(* FIXME: Move *)
+
+Definition get_var {A} (mg ml : Pmap A) (mr : list A) (v : var) : option A :=
+  match v with
+  | rel r => mr !! (r :> nat)
+  | loc l => ml !! l
+  | glob g => mg !! g
+  end.
+
+
+
+Fixpoint te_substl (f : Idx -> var) (te : tensorexpr) : tensorexpr :=
+  match te with
+  | tone => tone
+  | tabstract abs low up =>
+    tabstract abs ((λ v, from_option f v (v2loc v)) <$> low)
+      ((λ v, from_option f v (v2loc v)) <$> up)
+  | tproduct l r =>
+    tproduct (te_substl f l) (te_substl f r)
+  | tsum ty smd =>
+    tsum ty (te_substl (addrel 1 ∘ f) smd)
+  end.
+
+
+
+
+
+
+
+
+
+
+
+
+
+
+Lemma withrelshift_0 f :
+  pointwise_relation var eq (withrelshift 0 f) f.
+Proof.
+  now intros []; cbv; case_match.
+Qed.
+
+
+Add Parametric Morphism : te_substl with signature
+  pointwise_relation _ eq ==> eq ==> eq as te_substl_ext.
+Proof.
+  intros f g Hfg te.
+  revert f g Hfg; induction te; intros f g Hfg.
+  - easy.
+  - cbn.
+    f_equal; apply list_fmap_ext; intros _ [] _; easy + cbn; apply Hfg.
+  - cbn; f_equal; auto.
+  - cbn.
+    f_equal.
+    apply IHte.
+    intros ?.
+    cbn.
+    now rewrite Hfg.
+Qed.
+
+Lemma elem_of_te_local_varset_tabstract absidx lower upper l :
+  l ∈ te_local_varset (tabstract absidx lower upper) <->
+  loc l ∈ lower ++ upper.
+Proof.
+  cbn.
+  rewrite elem_of_list_to_set, elem_of_list_omap.
+  split; [|unfold v2loc; eexists; split; [eauto|reflexivity]].
+  now intros ([] & ? & [= ->]).
+Qed.
+
+
+
+Lemma relabel_te_ext f g te :
+  pointwise_relation var eq f g ->
+  relabel_te f te = relabel_te g te.
+Proof.
+  intros; now apply relabel_te_aux_ext.
+Qed.
+
+Lemma withrelshift_compose shift f g v :
+  withrelshift shift f (withrelshift shift g v) =
+  withrelshift shift (f ∘ g) v.
+Proof.
+  destruct v; cbn; [|destruct (g _); cbn; [rewrite decide_False by lia;
+    repeat first [lia | f_equal] |reflexivity..]..].
+  case_decide.
+  - cbn; now apply decide_True.
+  - destruct (g _); [|reflexivity..].
+    cbn.
+    rewrite decide_False by lia.
+    repeat first [lia | f_equal].
+Qed.
+
+
+Lemma withrelshift_id shift v :
+  withrelshift shift id v = v.
+Proof.
+  destruct v; [|reflexivity..].
+  cbn.
+  case_decide; f_equal; lia.
+Qed.
+
+Lemma relabel_te_aux_compose shift f g te :
+  relabel_te_aux shift g (relabel_te_aux shift f te) =
+  relabel_te_aux shift (g ∘ f) te.
+Proof.
+  revert shift; induction te; intros shift.
+  - reflexivity.
+  - cbn.
+    rewrite <- ! list_fmap_compose.
+    f_equal; apply list_fmap_ext; intros _ v _;
+    cbn; apply withrelshift_compose.
+  - cbn; f_equal; auto.
+  - cbn.
+    f_equal.
+    auto.
+Qed.
+
+Lemma relabel_te_compose f g te :
+  relabel_te g (relabel_te f te) = relabel_te (g ∘ f) te.
+Proof.
+  apply relabel_te_aux_compose.
+Qed.
+
+
+Lemma relabel_te_aux_id shift te :
+  relabel_te_aux shift id te =
+  te.
+Proof.
+  revert shift; induction te; intros shift.
+  - reflexivity.
+  - cbn.
+    now rewrite 2 list_fmap_id' by now intros; apply withrelshift_id.
+  - cbn; f_equal; auto.
+  - cbn.
+    f_equal.
+    auto.
+Qed.
+
+Lemma relabel_te_id te :
+  relabel_te id te = te.
+Proof.
+  apply relabel_te_aux_id.
+Qed.
+
+
+
+
+
+
+
+
+
+
+
+
+
+
+
+
+
+
+
+(* TODO: Rewrite condition: te_local_varset lhs ⊆ te_local_varset rhs *)
+
+Lemma extend_map_of_abstract_pair_correct
+  (mb mbi : Pmap Idx) (* The map and inverse map of [rel]/bound variables,
+    which must map to other bound variables *)
+  (ml : Pmap var) (* The map of local variables, which can map to any [var] *)
+  (mlran : Pset) (* The set of [rel] variables in the range of [ml], which
+     must be disjoint from the image of [mb] / domain of [mbi] *)
+  (l r : list var)
+  mb' mbi' ml' mlran' :
+  extend_map_of_abstract_pair mb mbi ml mlran l r =
+    Some (mb', mbi', ml', mlran') ->
+  map_inverses mb mbi ->
+  set_Forall (λ r, mbi !! r = None) mlran ->
+  map_img (omap v2rel ml) = mlran ->
+  mb ⊆ mb' /\ mbi ⊆ mbi' /\ ml ⊆ ml' /\
+  map_inverses mb' mbi' /\
+  dom mb' = dom mb ∪ list_to_set (omap v2rel l) /\
+  set_Forall (λ r, mbi' !! r = None) mlran' /\
+  map_img (omap v2rel ml') = mlran' /\
+  dom ml' = dom ml ∪ list_to_set (omap v2loc l) /\
+  Some <$> r = (var_elim (fmap rel ∘ (mb' !!.)) (ml' !!.)
+     (λ g, Some (glob g))) <$> l.
+Proof.
+  revert r mb mbi ml mlran mb' mbi' ml' mlran';
+  induction l as [|hl l IHl]; intros [|hr r]; [|easy..|];
+  intros mb mbi ml mlran mb' mbi' ml' mlran';
+  [cbn; intros [= -> -> -> ->] **; split_and!; easy + set_solver +|].
+  cbn [extend_map_of_abstract_pair].
+  refine (match hl with
+    | rel rl => match hr with
+      | rel rr => _
+      | _ => fun H => False_rect _ (None_ne_Some _ H)
+      end
+    | loc ll => _
+    | glob gl =>
+      match hr with
+      | glob gr => _
+      | _ => fun H => False_rect _ (None_ne_Some _ H)
+      end
+    end).
+  - destruct (mb !! rl) as [rr'|] eqn:Hrr';
+    [|destruct (mbi !! rr) eqn:Hrl; [easy|]];
+    rewrite <- decide_bool_decide.
+    + case_decide as Heq; [|easy].
+      subst rr'.
+      intros Hext Hinvs Hdisj Hmlran.
+      apply IHl in Hext as Hs; [|eauto..].
+      split_and!; try apply Hs;
+        destruct Hs as (Hmb & Hmbi & Hml & Hinvs' & Hdoms & Hs).
+      * rewrite Hdoms.
+        cbn [omap list_omap v2rel list_to_set].
+        apply elem_of_dom_2 in Hrr'.
+        set_solver + Hrr'.
+      * f_equal /=; [|apply Hs].
+        apply (fun H => lookup_weaken _ _ _ _ H Hmb) in Hrr'.
+        now rewrite Hrr'.
+    + case_decide as Hrr_disj; [easy|].
+      intros Hext Hinvs Hdisj Hmlran.
+      specialize (IHl _ _ _ _ _ _ _ _ _ Hext).
+      tspecialize IHl by now apply map_inverses_insert_fresh.
+      tspecialize IHl by now
+        intros lr Hlr;
+        rewrite lookup_insert_ne by (now intros <-);
+        now apply Hdisj.
+      tspecialize IHl by easy.
+      split_and!; try apply IHl.
+      1: now rewrite <- IHl.1; apply insert_subseteq.
+      1: now rewrite <- IHl.2.1; apply insert_subseteq.
+      1: cbn [omap list_omap v2rel list_to_set];
+        rewrite IHl.2.2.2.2.1; set_solver +.
+      cbn; f_equal.
+      * specialize (IHl.1 rl).
+        cbn.
+        rewrite lookup_insert.
+        cbn.
+        destruct (mb' !! rl) as [|]; [|easy].
+        intros <-.
+        easy.
+      * destruct IHl as (Hmb & _ & Hml & _ & _ & _ & _ & _ & Hlr).
+        apply (list_eq_same_length) with (length r);
+        [apply (f_equal length) in Hlr; revert Hlr;
+          simpl_list; easy| now rewrite length_fmap|].
+        intros i mri mli Hi Heq.
+        pose proof Heq as Heq'.
+        rewrite list_lookup_fmap in Heq.
+        apply lookup_lt_is_Some in Hi as Hri.
+        destruct Hri as [ri Hri].
+        rewrite Hri in Heq.
+        cbn in Heq.
+        apply (inj Some) in Heq.
+        subst mri.
+        rewrite list_lookup_fmap.
+        rewrite Hlr in Heq'.
+        rewrite list_lookup_fmap in Heq'.
+        destruct (l !! i) as [li|]; [|easy].
+        cbn in Heq'.
+        apply (inj Some) in Heq'.
+        destruct li as [lr | ll | lg]; cbn in Heq' |- *;
+        now intros [= <-].
+  - destruct (ml !! ll) as [vr'|] eqn:Hvr';
+    [rewrite <- decide_bool_decide; case_decide as Heq; [|intros [=]]|
+    destruct hr as [rr|rl|rg] eqn:Hhr;
+    [destruct (mbi !! rr) eqn:Hmbirr;
+      [intros [=]|]|..]].
+    + intros Hext Hinvs Hdisj Hmlran.
+      specialize (IHl _ _ _ _ _ _ _ _ _ Hext).
+      do 3 tspecialize IHl by easy.
+      split_and!; try apply IHl.
+      * rewrite IHl.2.2.2.2.2.2.2.1.
+        cbn [omap list_omap v2loc list_to_set].
+        apply elem_of_dom_2 in Hvr'.
+        set_solver +Hvr'.
+      * destruct IHl as (Hmb & Hmbi & Hml & Hs).
+        f_equal /=; [|apply Hs].
+        subst.
+        now apply (fun H => lookup_weaken _ _ _ _ H Hml) in Hvr'.
+    + intros Hext Hinvs Hdisj Hmlran.
+      specialize (IHl _ _ _ _ _ _ _ _ _ Hext Hinvs).
+      tspecialize IHl. 1:{
+        apply set_Forall_union; [|easy].
+        now apply set_Forall_singleton.
+      }
+      tspecialize IHl. 1:{
+        rewrite omap_insert.
+        cbn [v2rel].
+        rewrite map_img_insert_notin_L, Hmlran; [easy|].
+        now rewrite lookup_omap, Hvr'.
+      }
+      split_and!; try apply IHl.
+      1: now rewrite <- IHl.2.2.1; apply insert_subseteq.
+      1: now rewrite IHl.2.2.2.2.2.2.2.1; set_solver +.
+      destruct IHl as (Hmb & Hmbi & Hml & Hs).
+      cbn; f_equal; [|apply Hs].
+      symmetry.
+      revert Hml.
+      apply lookup_weaken, lookup_insert.
+    + intros Hext Hinvs Hdisj Hmlran.
+      specialize (IHl _ _ _ _ _ _ _ _ _ Hext Hinvs Hdisj).
+      rewrite omap_insert_None in IHl by reflexivity.
+      rewrite delete_notin in IHl by now rewrite lookup_omap, Hvr'.
+      tspecialize IHl by easy.
+      subst hr.
+      split_and!; try apply IHl.
+      1: now rewrite <- IHl.2.2.1; apply insert_subseteq.
+      1: now rewrite IHl.2.2.2.2.2.2.2.1; set_solver +.
+      destruct IHl as (Hmb & Hmbi & Hml & Hs).
+      cbn; f_equal; [|apply Hs].
+      symmetry.
+      revert Hml.
+      apply lookup_weaken, lookup_insert.
+    + intros Hext Hinvs Hdisj Hmlran.
+      specialize (IHl _ _ _ _ _ _ _ _ _ Hext Hinvs Hdisj).
+      rewrite omap_insert_None in IHl by reflexivity.
+      rewrite delete_notin in IHl by now rewrite lookup_omap, Hvr'.
+      tspecialize IHl by easy.
+      subst hr.
+      split_and!; try apply IHl.
+      1: now rewrite <- IHl.2.2.1; apply insert_subseteq.
+      1: now rewrite IHl.2.2.2.2.2.2.2.1; set_solver +.
+      destruct IHl as (Hmb & Hmbi & Hml & Hs).
+      cbn; f_equal; [|apply Hs].
+      symmetry.
+      revert Hml.
+      apply lookup_weaken, lookup_insert.
+  - rewrite <- decide_bool_decide.
+    case_decide as Hgs; [|easy].
+    intros Hext Hinvs Hdisj Hmlran.
+    specialize (IHl _ _ _ _ _ _ _ _ _ Hext Hinvs Hdisj Hmlran).
+    split_and!; try apply IHl.
+    f_equal /=; [now subst|].
+    apply IHl.
+Qed.
+
+
+Lemma list_first_omap_eq_head_bind {A B} (f : A -> option B) l :
+  list_first_omap f l =
+  head (x ← l; from_option (λ x, [x]) [] (f x)).
+Proof.
+  induction l; [done|].
+  cbn.
+  rewrite IHl.
+  destruct (f a); reflexivity.
+Qed.
+
+Lemma list_first_omap_Some {A B} (f : A -> option B) l b :
+  list_first_omap f l = Some b ->
+  exists a, a ∈ l /\ f a = Some b.
+Proof.
+  rewrite list_first_omap_eq_head_bind.
+  intros (a & Hb & Ha)%head_Some_elem_of%elem_of_list_bind.
+  exists a; split; [easy|].
+  destruct (f a); [|easy].
+  cbn in Hb.
+  rewrite elem_of_list_singleton in Hb.
+  now subst.
+Qed.
+
+
+
+
+
+Lemma extend_match_of_abstract_tensors_correct
+  (P : Pmap Idx -> Pmap Idx -> Pmap var -> Pset ->
+    list (Idx * list var * list var) -> Prop)
+  `{HP : forall mb mbi ml mlran rrest, Decision (P mb mbi ml mlran rrest)}
+  (mb mbi : Pmap Idx) (* The map and inverse map of [rel]/bound variables,
+    which must map to other bound variables *)
+  (ml : Pmap var) (* The map of local variables, which can map to any [var] *)
+  (mlran : Pset) (* The set of [rel] variables in the range of [ml], which
+     must be disjoint from the image of [mb] / domain of [mbi] *)
+  (labs rabs : list (Idx * list var * list var))
+  mb' mbi' ml' mlran' rrest :
+
+  extend_match_of_abstract_tensors P mb mbi ml mlran labs rabs =
+    Some (mb', mbi', ml', mlran', rrest) ->
+
+    map_inverses mb mbi ->
+  set_Forall (λ r, mbi !! r = None) mlran ->
+  map_img (omap v2rel ml) = mlran ->
+  P mb' mbi' ml' mlran' rrest /\
+  mb ⊆ mb' /\ mbi ⊆ mbi' /\ ml ⊆ ml' /\
+  map_inverses mb' mbi' /\
+  dom mb' = dom mb ∪ abstracts_rel_vars labs /\
+  set_Forall (λ r, mbi' !! r = None) mlran' /\
+  map_img (omap v2rel ml') = mlran' /\
+  dom ml' = dom ml ∪ abstracts_local_vars labs /\
+  (relabel_abs (var_elim (fmap rel ∘ (mb' !!.)) (ml' !!.)
+     (λ g, Some (glob g))) <$> labs) ++
+     (relabel_abs Some <$> rrest) ≡ₚ relabel_abs Some <$> rabs.
+Proof.
+  revert rabs mb mbi ml mlran mb' mbi' ml' mlran' rrest;
+  induction labs as [|((fl, lowl), upl) labs IHlabs];
+  intros rabs mb mbi ml mlran mb' mbi' ml' mlran' rrest;
+  [cbn; case_decide; intros [= -> -> -> -> ->] **; split_and!;
+    easy + set_solver +|].
+  cbn.
+  intros ((((absr, lowr), upr), rrest') &
+    (Habsr & Hperm)%elem_of_list_select_perm_Prop
+    & ([[[mb1 mbi1] ml1] mlran1] & Hext1 &
+      ([[[mb2 mbi2] ml2] mlran2] & Hext2 & Hext)%bind_Some
+      )%bind_Some)%list_first_omap_Some.
+  intros Invs Hdisj Hmlran.
+  specialize (extend_map_of_abstract_pair_correct _ _ _ _ _ _
+    _ _ _ _ Hext1) as Hext1'.
+  clear Hext1; rename Hext1' into Hext1.
+  tspecialize Hext1 by auto.
+  tspecialize Hext1 by auto.
+  tspecialize Hext1 by auto.
+  specialize (extend_map_of_abstract_pair_correct _ _ _ _ _ _
+    _ _ _ _ Hext2) as Hext2'.
+  clear Hext2; rename Hext2' into Hext2.
+  tspecialize Hext2 by apply Hext1.
+  tspecialize Hext2 by apply Hext1.
+  tspecialize Hext2 by apply Hext1.
+  specialize (IHlabs _ _ _ _ _ _ _ _ _ _ Hext).
+  move IHlabs at bottom.
+  tspecialize IHlabs by apply Hext2.
+  tspecialize IHlabs by apply Hext2.
+  tspecialize IHlabs by apply Hext2.
+  split; [apply IHlabs|].
+  split; [now rewrite Hext1.1, Hext2.1|].
+  split; [now rewrite Hext1.2.1, Hext2.2.1|].
+  split; [now rewrite Hext1.2.2.1, Hext2.2.2.1|].
+  split; [apply IHlabs|].
+  split.
+  1: {
+    rewrite IHlabs.2.2.2.2.2.1, Hext2.2.2.2.2.1, Hext1.2.2.2.2.1.
+    rewrite list_to_set_app_L.
+    rewrite omap_app, list_to_set_app_L.
+    set_solver +.
+  }
+  split; [apply IHlabs|].
+  split; [apply IHlabs|].
+  split.
+  1: {
+    rewrite IHlabs.2.2.2.2.2.2.2.2.1,
+      Hext2.2.2.2.2.2.2.2.1, Hext1.2.2.2.2.2.2.2.1.
+    rewrite list_to_set_app_L.
+    rewrite omap_app, list_to_set_app_L.
+    set_solver +.
+  }
+
+  rewrite Hperm.
+  cbn.
+  rewrite <- IHlabs.2.2.2.2.2.2.2.2.2.
+  cbn.
+  f_equiv.
+  f_equal; [f_equal; [easy|]|].
+  - pose proof Hext1.2.2.2.2.2.2.2.2 as Hlowl.
+    apply list_eq_same_length with (length lowl);
+    [generalize (f_equal length Hlowl); now simpl_list|
+    now rewrite length_fmap|].
+    intros i x y Hi.
+    rewrite 2!list_lookup_fmap.
+    generalize (f_equal (.!! i) Hlowl).
+    rewrite 2!list_lookup_fmap.
+    destruct (lowl !! i) as [li|]; [|easy].
+    destruct (lowr !! i) as [ri|]; [|easy].
+    cbn in *.
+    intros [= Hli] [= <-] [= <-].
+    destruct li as [lr | ll | lg]; cbn in *;
+    rewrite Hli; [f_equal | | reflexivity].
+    + destruct (mb1 !! lr) as [mb1lr|] eqn:Hmb1lr ; [|easy].
+      apply (lookup_weaken _ _ _ _ (Hmb1lr)).
+      rewrite Hext2.1; apply IHlabs.2.1.
+    + destruct (ml1 !! ll) as [ml1ll|] eqn:Hml1ll ; [|easy].
+      apply (lookup_weaken _ _ _ _ (Hml1ll)).
+      rewrite Hext2.2.2.1; apply IHlabs.2.2.2.1.
+  - pose proof Hext2.2.2.2.2.2.2.2.2 as Hupl.
+    apply list_eq_same_length with (length upl);
+    [generalize (f_equal length Hupl); now simpl_list|
+    now rewrite length_fmap|].
+    intros i x y Hi.
+    rewrite 2!list_lookup_fmap.
+    generalize (f_equal (.!! i) Hupl).
+    rewrite 2!list_lookup_fmap.
+    destruct (upl !! i) as [li|]; [|easy].
+    destruct (upr !! i) as [ri|]; [|easy].
+    cbn in *.
+    intros [= Hli] [= <-] [= <-].
+    destruct li as [lr | ll | lg]; cbn in *;
+    rewrite Hli; [f_equal | | reflexivity].
+    + destruct (mb2 !! lr) as [mb1lr|] eqn:Hmb1lr ; [|easy].
+      apply (lookup_weaken _ _ _ _ (Hmb1lr)).
+      apply IHlabs.2.1.
+    + destruct (ml2 !! ll) as [ml1ll|] eqn:Hml1ll ; [|easy].
+      apply (lookup_weaken _ _ _ _ (Hml1ll)).
+      apply IHlabs.2.2.2.1.
+Qed.
+
+
+
+
+
+
+(* Typing for [tensorexpr]s *)
+
+Notation vartypecontext := (Pmap Ty).
+Notation abstypecontext := (Pmap (list Ty)).
+
+Record typecontext := mk_tc {
+  tc_ma : abstypecontext;
+  tc_mg : vartypecontext;
+  tc_ml : vartypecontext;
+  tc_mr : list Ty;
+}.
+
+Definition tc_cons_type (ty : Ty) (tc : typecontext) : typecontext :=
+  mk_tc (tc.(tc_ma)) (tc.(tc_mg)) (tc.(tc_ml)) (ty :: tc.(tc_mr)).
+
+Definition tc_get_var (tc : typecontext) (v : var) : option Ty :=
+  get_var (tc.(tc_mg)) (tc.(tc_ml)) (tc.(tc_mr)) v.
+
+Definition tc_app_types (tys : list Ty) (tc : typecontext) : typecontext :=
+  mk_tc (tc.(tc_ma)) (tc.(tc_mg)) (tc.(tc_ml)) (tys ++ tc.(tc_mr)).
+
+Lemma tc_cons_app_type ty tys tc :
+  tc_cons_type ty (tc_app_types tys tc) = tc_app_types (ty :: tys) tc.
+Proof.
+  reflexivity.
+Qed.
+
+(* FIXME: Move *)
+Definition tc_eqn_with_locals (tc : typecontext) (tl : Pmap Ty) : typecontext :=
+  mk_tc (tc.(tc_ma)) (tc.(tc_mg)) (tl ∪ tc.(tc_ml)) [].
+
+Declare Scope tensorexpr_scope.
+Delimit Scope tensorexpr_scope with te.
+Bind Scope tensorexpr_scope with tensorexpr.
+
+Declare Custom Entry args_print.
+
+Declare Custom Entry var_print.
+
+Notation " '#' r " := (rel r) (in custom var_print at level 1).
+Notation " 'L@' l " := (loc l) (in custom var_print at level 1).
+Notation " 'G@' g " := (glob g) (in custom var_print at level 1).
+
+Notation " '()' " := (@nil var) (in custom args_print at level 0).
+Notation " '(' x ,  .. ,  y ')'" :=
+  (cons x .. (cons y nil) ..)
+  (in custom args_print at level 0, x custom var_print at level 1,
+    y custom var_print at level 1).
+
+
+Notation "te  *  te'" := (tproduct te%te te'%te) : tensorexpr_scope.
+Notation "1" := (tone) : tensorexpr_scope.
+Notation "∑'  ty ,  te" := (tsum ty%nat te%te)
+  (at level 45, right associativity) : tensorexpr_scope.
+Notation "'!{' f '}'  low  up" :=
+  (tabstract f low up) (at level 10,
+    low custom args_print at level 0,
+    up custom args_print at level 0) : tensorexpr_scope.
+
+
+
+Fixpoint well_typed (tc : typecontext) (te : tensorexpr) : Prop :=
+  match te with
+  | tone => True
+  | tabstract f low up =>
+    (fmap Some) <$> tc.(tc_ma) !! f = Some ((tc_get_var tc) <$> (low ++ up))
+  | tproduct te te' =>
+    well_typed tc te /\ well_typed tc te'
+  | tsum ty te => well_typed (tc_cons_type ty tc) te
+  end.
+
+
+Definition is_well_typed_abs (ta : abstypecontext)
+  (tg tl : vartypecontext) (tr : list Ty)
+  (f : Idx) (low up : list var) : bool :=
+  bool_decide ((fmap Some) <$> ta !! f =@{option (list _)}
+    Some ((get_var tg tl tr) <$> (low ++ up))).
+
+Fixpoint is_well_typed (ta : abstypecontext)
+  (tg tl : vartypecontext) (tr : list Ty) (te : tensorexpr) : bool :=
+  match te with
+  | tone => true
+  | tabstract f low up => is_well_typed_abs ta tg tl tr f low up
+  | tproduct te te' => is_well_typed ta tg tl tr te && is_well_typed ta tg tl tr te'
+  | tsum ty te => is_well_typed ta tg tl (ty :: tr) te
+  end.
+
+Lemma is_well_typed_correct tc te :
+  is_well_typed (tc.(tc_ma)) (tc.(tc_mg)) (tc.(tc_ml)) (tc.(tc_mr)) te <->
+  well_typed tc te.
+Proof.
+  destruct tc as [ta tg tl tr]; cbn.
+  revert tr; induction te; intros tr; cbn.
+  - easy.
+  - apply bool_decide_spec.
+  - now rewrite andb_True, IHte1, IHte2.
+  - apply IHte.
+Qed.
+
+Lemma is_well_typed_correct_alt tc te :
+  if (is_well_typed (tc.(tc_ma)) (tc.(tc_mg)) (tc.(tc_ml)) (tc.(tc_mr)) te)
+  then well_typed tc te else ¬ well_typed tc te.
+Proof.
+  specialize (is_well_typed_correct tc te).
+  destruct (is_well_typed _ _ _ _ _); cbn; naive_solver.
+Qed.
+
+#[global] Instance well_typed_dec tc te : Decision (well_typed tc te) :=
+  match is_well_typed (tc.(tc_ma)) (tc.(tc_mg)) (tc.(tc_ml)) (tc.(tc_mr)) te
+    as b return ((if b return Prop then _ else _) -> _) with
+  | true => left
+  | false => right
+  end (is_well_typed_correct_alt tc te).
+
+
+Definition all_bound (tl : tensorlist) : Prop :=
+  abstracts_rel_vars tl.(tl_abstracts) =
+  list_to_set (pseq 1 (lengthN tl.(tl_sums))).
+
+Definition tleq_well_typed tc teeq : Prop :=
+  let tc' := mk_tc tc.(tc_ma) tc.(tc_mg) teeq.(tleq_univ) [] in
+  well_typed tc' teeq.(tleq_lhs) /\
+  well_typed tc' teeq.(tleq_rhs) /\
+  te_local_varset teeq.(tleq_rhs) ⊆ te_local_varset teeq.(tleq_lhs) /\
+  dom teeq.(tleq_univ) = te_local_varset teeq.(tleq_lhs)
+    (* NB: ⊆ suffices, by the first WT condition *).
+
+(* (* TODO: Make; FIXME: Move *)
+Fixpoint Pmap_ne_sizeP {A} (p : Pmap_ne A) : positive := *)
+  
+
+
+Local Open Scope lazy_bool_scope.
+Definition tleq_is_well_typed_aux ta tg lhs rhs univ :=
+  let '(mk_tl lsums labs) := lhs in
+  let '(mk_tl rsums rabs) := rhs in
+  let lhs_mr := reverse lsums in
+  let rhs_mr := reverse rsums in
+  (forallb (λ '(f, low, up),
+    is_well_typed_abs ta tg univ lhs_mr f low up) labs &&&
+  forallb (λ '(f, low, up),
+    is_well_typed_abs ta tg univ rhs_mr f low up) rabs &&&
+  let llocs := abstracts_local_vars labs in
+  Pset_subseteqb (abstracts_local_vars rabs) llocs &&&
+  Pmap_dom_subseteqb univ (llocs.(mapset.mapset_car))
+  ).
+
+Lemma is_well_typed_tproducts ta tg tl tr tes :
+  is_well_typed ta tg tl tr (tproducts tes) =
+  forallb (is_well_typed ta tg tl tr) tes.
+Proof.
+  induction tes as [|te tes]; cbn; [easy|rewrite <- IHtes].
+  f_equal.
+  destruct tes; [|easy].
+  cbn; now rewrite andb_true_r.
+Qed.
+
+Lemma tl_is_well_typed_alt_aux ta tg tl tr (tel : tensorlist) :
+  is_well_typed ta tg tl tr tel =
+    let '(mk_tl lsums labs) := tel in
+    forallb (λ '(f, low, up),
+    is_well_typed_abs ta tg tl (rev_append lsums tr) f low up) labs.
+Proof.
+  destruct tel as [lsums labs].
+  revert tr; induction lsums; intros tr.
+  - cbn.
+    rewrite is_well_typed_tproducts.
+    apply Bool.eq_iff_eq_true;
+    rewrite 2 forallb_forall, <- 2 List.Forall_forall.
+    rewrite Forall_fmap.
+    apply Forall_iff.
+    intros ((f, low), up); reflexivity.
+  - cbn.
+    apply IHlsums.
+Qed.
+
+Lemma well_typed_local_varset_subseteq tc te :
+  well_typed tc te -> te_local_varset te ⊆ dom (tc.(tc_ml)).
+Proof.
+  revert tc;
+  induction te; intros tc.
+  - easy.
+  - cbn.
+    destruct (tc_ma tc !! _) as [tys|]; [cbn|easy].
+    generalize (lower ++ upper); intros vs.
+    intros [= Hvs].
+    revert tys Hvs;
+    induction vs as [|v vs IHvs];
+    [easy|intros [|ty tys] [= Hv Hvs%IHvs]].
+    cbn.
+    destruct v as [|l|]; [apply Hvs| |apply Hvs].
+    simpl.
+    cbn in Hv.
+    symmetry in Hv.
+    apply elem_of_dom_2 in Hv.
+    set_solver + Hv Hvs.
+  - cbn; set_solver.
+  - cbn.
+    apply IHte.
+Qed.
+
+Lemma and_iff_from_l {P Q R S} :
+  (P <-> Q) -> (P -> Q -> (R <-> S)) ->
+  P /\ R <-> Q /\ S.
+Proof.
+  tauto.
+Qed.
+
+Lemma te_local_varset_tl (tl : tensorlist) :
+  te_local_varset tl =
+  abstracts_local_vars tl.(tl_abstracts).
+Proof.
+  destruct tl as [sums abs].
+  cbn.
+  induction sums; [|apply IHsums].
+  cbn.
+  induction abs as [|((f, low), up) abs IHabs]; [reflexivity|].
+  cbn.
+  rewrite list_to_set_app_L, <- IHabs.
+  destruct abs as [|((f', low'), up') abs]; cbn.
+  - now rewrite union_empty_r_L.
+  - reflexivity.
+Qed.
+
+
+Lemma tleq_is_well_typed_aux_correct ta tg tl tr lhs rhs univ :
+  tleq_is_well_typed_aux ta tg lhs rhs univ <->
+  tleq_well_typed (mk_tc ta tg tl tr) (mk_tleq lhs rhs univ).
+Proof.
+  unfold tleq_is_well_typed_aux, tleq_well_typed; cbn.
+  destruct lhs as [lsums labs], rhs as [rsums rabs].
+  rewrite 3 lazy_andb_True, <- (and_assoc _).
+  apply and_iff_from_l;
+    [now rewrite <- is_well_typed_correct, tl_is_well_typed_alt_aux|].
+  intros Hall_l Hty_l.
+  apply and_iff_from_l;
+    [now rewrite <- is_well_typed_correct, tl_is_well_typed_alt_aux|].
+  intros Hall_r Hty_r.
+  apply and_iff_from_l;
+    [now rewrite Pset_subseteqb_correct, 2 te_local_varset_tl|].
+  intros Hsub%Pset_subseteqb_correct Hsub'.
+  rewrite Pmap_dom_subseteqb_correct, Aux_stdpp.dom_Pset.
+  rewrite te_local_varset_tl; cbn [tl_abstracts].
+  split; [|now intros ->].
+  intros Hsub''.
+  unfold_leibniz.
+  apply set_subseteq_antisymm; [easy|].
+  apply well_typed_local_varset_subseteq in Hty_l.
+  rewrite te_local_varset_tl in Hty_l.
+  apply Hty_l.
+Qed.
+
+
+Lemma pos_swap_alt p :
+  pos_swap p = (if decide (p = 1) then 2 else if decide (p = 2) then 1 else p)%positive.
+Proof.
+  unfold pos_swap.
+  destruct p as [| []|]; reflexivity.
+Qed.
+
+
+Lemma relabel_te_swap_wt_aux ctx prefix ty ty' te :
+  well_typed {|
+    tc_ma := tc_ma ctx;
+    tc_mg := tc_mg ctx;
+    tc_ml := tc_ml ctx;
+    tc_mr := prefix ++ ty' :: ty :: tc_mr ctx
+  |} te
+  -> well_typed {|
+      tc_ma := tc_ma ctx;
+      tc_mg := tc_mg ctx;
+      tc_ml := tc_ml ctx;
+      tc_mr := prefix ++ ty :: ty' :: tc_mr ctx
+    |}
+    (relabel_te_aux (lengthN prefix) (relabel_rels pos_swap) te).
+Proof.
+  revert prefix; induction te; intros prefix; cbn.
+  - easy.
+  - intros ->.
+    f_equal.
+    rewrite <- fmap_app, <- list_fmap_compose.
+    apply list_fmap_ext; intros _ v _.
+    destruct v; [|easy..].
+    cbn.
+    case_decide as Hle; cbn.
+    + rewrite 2 lookup_app_l by now
+        rewrite <- lengthN_correct; lia.
+      reflexivity.
+    + rewrite 2 lookup_app_r by now
+        rewrite <- lengthN_correct; lia.
+      rewrite pos_swap_alt.
+      case_decide as H1; [|case_decide as H2].
+      * replace (_ - _)%nat with 0%nat by
+          now rewrite <- lengthN_correct; lia.
+        replace (_ - _)%nat with 1%nat by
+          now rewrite <- lengthN_correct; lia.
+        reflexivity.
+      * replace (_ - _)%nat with 1%nat by
+          now rewrite <- lengthN_correct; lia.
+        replace (_ - _)%nat with 0%nat by
+          now rewrite <- lengthN_correct; lia.
+        reflexivity.
+      * symmetry.
+        replace (_ - _)%nat with (pos_to_nat_pred p - length prefix)%nat by lia.
+        enough (Hge : (pos_to_nat_pred p - length prefix >= 2)%nat) by
+          now clear -Hge; rewrite ! lookup_cons_ne_0 by lia.
+        rewrite <- lengthN_correct; lia.
+  - intros []; auto.
+  - unfold tc_cons_type; cbn.
+    rewrite app_comm_cons.
+    apply IHte.
+Qed.
+
+Lemma relabel_te_swap_wt ctx ty ty' te :
+  well_typed (tc_cons_type ty' (tc_cons_type ty ctx)) te
+  -> well_typed (tc_cons_type ty (tc_cons_type ty' ctx))
+    (relabel_te (relabel_rels pos_swap) te).
+Proof.
+  rewrite (unfold relabel_te).
+  unfold tc_cons_type; cbn.
+  change (ty' :: ty :: ?x) with ([] ++ ty' :: ty :: x).
+  change (ty :: ty' :: ?x) with ([] ++ ty :: ty' :: x).
+  remember nil as prefix eqn:Hpre.
+  replace 0%N with (lengthN prefix) by now subst.
+  clear Hpre.
+  apply relabel_te_swap_wt_aux.
+Qed.
+
+
+
+Lemma relabel_te_cons_wt_aux ctx pre tys te :
+  well_typed {|
+      tc_ma := tc_ma ctx;
+      tc_mg := tc_mg ctx;
+      tc_ml := tc_ml ctx;
+      tc_mr := pre ++ tc_mr ctx
+    |} te <->
+  well_typed {|
+      tc_ma := tc_ma ctx;
+      tc_mg := tc_mg ctx;
+      tc_ml := tc_ml ctx;
+      tc_mr := pre ++ tys ++ tc_mr ctx
+    |} (relabel_te_aux (lengthN pre) (relabel_rels (λ p, pos_add_N p (lengthN tys))) te).
+Proof.
+  revert tys pre.
+  induction te; intros tys pre.
+  - easy.
+  - cbn.
+    f_equiv.
+    f_equal.
+    rewrite <- fmap_app, <- list_fmap_compose.
+    apply list_fmap_ext; intros _ v _.
+    destruct v; [|easy..].
+    cbn.
+    case_decide as Hle; cbn.
+    + rewrite 2 lookup_app_l by now
+        rewrite <- lengthN_correct; lia.
+      reflexivity.
+    + rewrite 2 lookup_app_r by now
+        rewrite <- lengthN_correct; lia.
+      rewrite <- lengthN_correct.
+      rewrite lookup_app_r by now rewrite <- lengthN_correct; lia.
+      f_equal.
+      rewrite <- lengthN_correct; lia.
+  - cbn; naive_solver.
+  - cbn. unfold tc_cons_type; cbn.
+    rewrite 2 app_comm_cons.
+    apply IHte.
+Qed.
+
+Lemma relabel_te_cons_wt ctx ty te :
+  well_typed ctx te <->
+  well_typed (tc_cons_type ty ctx) (relabel_te (relabel_rels Pos.succ) te).
+Proof.
+  rewrite (unfold relabel_te).
+  unfold tc_cons_type; cbn.
+  change (ty :: ?x) with ([] ++ ty :: x).
+  remember nil as prefix eqn:Hpre.
+  replace 0%N with (lengthN prefix) by now subst.
+  (* intros Hwt. *)
+  erewrite relabel_te_aux_ext;
+  [| | reflexivity]; [etransitivity; [|apply (relabel_te_cons_wt_aux _ _ [ty])]|];
+  [|intros []; [|reflexivity..]; cbn; f_equal; lia].
+  subst.
+  now destruct ctx.
+Qed.
+
+
+
+Lemma te_substl_wt_aux ctx rels tys te (substs : Pmap var) :
+  (forall l, l ∈ te_local_varset te ->
+    (tc_get_var ctx) <$> (substs !! l) = (Some <$> tys !! l)) ->
+  well_typed (tc_app_types rels (tc_eqn_with_locals ctx tys)) te ->
+  well_typed (tc_app_types rels ctx)
+    (te_substl (addrel (lengthN rels) ∘ λ l, default (loc l) (substs !! l)) te).
+Proof.
+  revert rels ctx;
+  induction te; intros rels ctx Hty.
+  - easy.
+  - cbn.
+    intros Hhyp.
+    assert (Hrels : forall r, rel r ∈ lower ++ upper -> (N.pos r <= lengthN rels)%N). 1:{
+      apply fmap_Some in Hhyp as (argtys & _ & Heq).
+      intros r (i & Hlui)%elem_of_list_lookup_1.
+      apply (f_equal (.!! i)) in Heq.
+      rewrite 2 list_lookup_fmap, Hlui in Heq.
+      cbn in Heq.
+      rewrite app_nil_r in Heq.
+      destruct (argtys !! i); [|easy].
+      cbn in Heq.
+      injection Heq.
+      intros ?%lookup_lt_Some.
+      rewrite lengthN_correct_rev.
+      lia.
+    }
+    revert Hhyp.
+    intros ->.
+    setoid_rewrite elem_of_te_local_varset_tabstract in Hty.
+    f_equal.
+    rewrite <- fmap_app, <- list_fmap_compose.
+    apply list_fmap_ext; intros _ v Hv%elem_of_list_lookup_2.
+    destruct v as [r|l|]; [..|reflexivity].
+    + cbn.
+      apply Hrels in Hv.
+      rewrite lengthN_correct_rev in Hv.
+      now rewrite 2 lookup_app_l by lia.
+    + cbn.
+      specialize (Hty l Hv).
+      rewrite lookup_union.
+      destruct (substs !! l), (tys !! l); try easy; cbn in *.
+      * rewrite union_Some_l.
+        revert Hty; intros [= <-].
+        unfold tc_get_var; cbn.
+        destruct v; [|reflexivity..].
+        cbn.
+        rewrite lengthN_correct_rev.
+        rewrite lookup_app_r by lia.
+        f_equal; lia.
+      * now rewrite option_union_left_id.
+  - cbn; intros [?%IHte1 ?%IHte2]; [|set_solver +Hty..].
+    now split.
+  - cbn.
+    intros Hte.
+    erewrite (te_substl_ext _
+      (addrel (N.succ (lengthN rels)) ∘ λ l, default (loc l) (substs !! l)));
+      [| | reflexivity].
+    2: {
+      intros v; cbn.
+      destruct (substs !! v) as [[]|]; [|reflexivity..].
+      cbn.
+      f_equal; lia.
+    }
+    rewrite tc_cons_app_type.
+    apply (IHte (ty :: rels)); [easy|].
+    now rewrite tc_cons_app_type in Hte.
+Qed.
+
+Lemma te_substl_wt ctx tys te (substs : Pmap var) :
+  (forall l, l ∈ te_local_varset te ->
+    (tc_get_var ctx) <$> (substs !! l) = (Some <$> tys !! l)) ->
+  well_typed (tc_eqn_with_locals ctx tys) te ->
+  well_typed ctx
+    (te_substl (λ l, default (loc l) (substs !! l)) te).
+Proof.
+  specialize (te_substl_wt_aux ctx [] tys te substs) as Hen.
+  intros Hty Hwt.
+  specialize (Hen Hty Hwt).
+  replace (tc_app_types _ _) with ctx in Hen by now destruct ctx.
+  erewrite te_substl_ext; [apply Hen | | reflexivity].
+  intros v; cbn.
+  destruct (substs !! v) as [[]|]; reflexivity.
+Qed.
+
+
+
+
+
+
+
+
+
+
+Fixpoint tl_to_te_with_aux (base : list tensorexpr) (sums : list Ty)
+  (abs : list (Idx * list var * list var)) : tensorexpr :=
+  match sums with
+  | [] => tproducts (base ++ (tabstract' <$> abs))
+  | ty :: sums => tsum ty (tl_to_te_with_aux base sums abs)
+  end.
+
+Notation tl_to_te_with base tl :=
+  (tl_to_te_with_aux base (tl_sums tl) (tl_abstracts tl)).
+
+Lemma tensorexpr_of_tensorlist_aux_to_tl_to_te_with_aux sums abs :
+  tensorexpr_of_tensorlist_aux sums abs =
+  tl_to_te_with_aux [] sums abs.
+Proof.
+  induction sums; cbn; congruence.
+Qed.
+
+
+
+(* Equivalence of [tensorlist]s up to (alpha-equivalence and) permutation *)
+Definition tl_aeq : relation tensorlist :=
+  fun tl tl' =>
+  exists (fr : Idx -> Idx),
+    let n := N.succ_pos (lengthN (tl.(tl_sums))) in
+    posperm n fr /\
+    ppermute fr (reverse tl.(tl_sums))
+      = (reverse tl'.(tl_sums)) /\
+    tl.(tl_abstracts) ≡ₚ
+      relabel_abs (relabel_rels $ make_pwf n fr) <$> tl'.(tl_abstracts).
+
+Lemma tl_aeq_refl tl : tl_aeq tl tl.
+Proof.
+  exists id.
+  split; [apply posperm_id|].
+  split; [apply ppermute_id|].
+  apply eq_reflexivity, symmetry, list_fmap_id'.
+  intros ((f, low), up) _.
+  cbn.
+  f_equal; [f_equal|]; apply list_fmap_id'; intros [] _; reflexivity ||
+    now cbn; case_decide.
+Qed.
+
+
+Lemma tl_aeq_symm tl tl' : tl_aeq tl tl' -> tl_aeq tl' tl.
+Proof.
+  intros (f & Hf & Hsums & Habs).
+  exists (posperm_inv (N.succ_pos $ lengthN tl.(tl_sums)) f).
+  apply (f_equal length) in Hsums as Hlen.
+  rewrite length_ppermute, 2 length_reverse in Hlen.
+  pose proof Hlen as HlenN.
+  rewrite <- 2 lengthN_correct in HlenN.
+  apply N2Nat.inj in HlenN.
+  intros n.
+  split; [subst n; rewrite <- HlenN; now apply posperm_inv_posperm|].
+  split.
+  - rewrite <- Hsums.
+    rewrite ppermute_compose by
+      now rewrite lengthN_reverse;
+        apply posperm_inv_bounded + apply posperm_bounded.
+    apply ppermute_id'.
+    rewrite lengthN_reverse.
+    intros p Hp.
+    now apply posperm_inv_rinv.
+  - rewrite Habs.
+    rewrite <- list_fmap_compose.
+    apply eq_reflexivity, symmetry, list_fmap_id'.
+    intros ((fidx, low), up) _.
+    cbn.
+    rewrite <- 2 list_fmap_compose.
+    f_equal; [f_equal|]; apply list_fmap_id'; intros [r| |] _; try reflexivity;
+      cbn;
+      subst n;
+      rewrite <- HlenN;
+      (destruct_decide (decide (N.succ_pos (lengthN tl.(tl_sums)) <= r)) as Hr;
+      [now rewrite decide_True |
+       rewrite decide_False by
+        now pose proof (posperm_bounded _ _ Hf r); lia]);
+    f_equal; apply posperm_inv_linv; easy + lia.
+Qed.
+
+Lemma tl_aeq_trans tl tl' tl'' : tl_aeq tl tl' -> tl_aeq tl' tl'' ->
+  tl_aeq tl tl''.
+Proof.
+  intros (f & Hf & Hfsums & Hfabs)
+    (g & Hg & Hgsums & Hgabs).
+  exists (f ∘ g).
+  intros n.
+  apply (f_equal length) in Hfsums as Hflen.
+  apply (f_equal length) in Hgsums as Hglen.
+  rewrite length_ppermute, !length_reverse in Hflen, Hglen.
+  pose proof Hflen as HflenN.
+  pose proof Hglen as HglenN.
+  rewrite <- 2 lengthN_correct in HflenN, HglenN.
+  apply N2Nat.inj in HflenN, HglenN.
+  split; [now apply posperm_compose; subst n; congruence|].
+  split.
+  - rewrite <- Hgsums, <- Hfsums.
+    symmetry; apply ppermute_compose;
+    rewrite lengthN_reverse;
+    now apply posperm_bounded; congruence.
+  - rewrite Hfabs, Hgabs.
+    rewrite <- list_fmap_compose.
+    apply eq_reflexivity.
+    apply list_fmap_ext; intros _ ((idx, low), up) _.
+    cbn.
+    rewrite <- 2 list_fmap_compose.
+    f_equal; [f_equal|]; apply list_fmap_ext; intros _ [r| |] _; try reflexivity;
+      cbn;
+      subst n;
+      rewrite <- HflenN;
+      (destruct_decide (decide (N.succ_pos (lengthN tl.(tl_sums)) <= r)) as Hr;
+      [now rewrite decide_True |
+       now rewrite decide_False by
+        now pose proof (posperm_bounded _ _ Hg r); lia]).
+Qed.
+
+Add Parametric Relation : tensorlist tl_aeq
+  reflexivity proved by tl_aeq_refl
+  symmetry proved by tl_aeq_symm
+  transitivity proved by tl_aeq_trans
+  as tl_aeq_setoid.
+
+(* TODO: This ^ gives us the proper definition of semantic tensorexpr equality *)
+
+(* TODO: Unused variables!!! *)
+
+Lemma tl_times_tlone_l tl : tl_times tlone tl = tl.
+Proof.
+  destruct tl as [sums abs]; cbn.
+  now case_match.
+Qed.
+
+Lemma tl_times_tlone_r tl : tl_times tl tlone = tl.
+Proof.
+  destruct tl as [sums abs]; cbn.
+  now case_match;
+  rewrite 2 app_nil_r.
+Qed.
+
+Lemma tensorlist_of_tensorexpr_tproducts tes :
+  tensorlist_of_tensorexpr (tproducts tes) =
+  fold_right tl_times tlone (tensorlist_of_tensorexpr <$> tes).
+Proof.
+  induction tes as [|te tes IHtes]; [reflexivity|].
+  cbn.
+  rewrite <- IHtes.
+  destruct tes; [|reflexivity].
+  cbn.
+  now rewrite tl_times_tlone_r.
+Qed.
+
+Lemma tensorlist_of_tl_to_te_with_aux tes sums abs :
+  tensorlist_of_tensorexpr (tl_to_te_with_aux tes sums abs) =
+  tl_app_sums sums $
+  fold_right tl_times (mk_tl [] abs) (tensorlist_of_tensorexpr <$> tes).
+Proof.
+  induction sums.
+  - cbn.
+    rewrite tensorlist_of_tensorexpr_tproducts.
+    rewrite fmap_app, fold_right_app.
+    f_equal.
+    induction abs as [|((f, low), up)]; [reflexivity|cbn].
+    rewrite IHabs.
+    cbn.
+    reflexivity.
+  - cbn.
+    now rewrite IHsums.
+Qed.
+
+
+Infix "=tl=" := tl_aeq (at level 70).
+
+(* FIXME: Move *)
+Lemma abs_fmap_l_ext {A} (idx : Idx) (f f' : A -> var) (low : list A) up up' :
+  (f <$> low) ++ up = (f' <$> low) ++ up' ->
+  (idx, f <$> low, up) = (idx, f' <$> low, up').
+Proof.
+  intros Heq%app_inj_len_l; [|now simpl_list].
+  destruct Heq;
+  congruence.
+Qed.
+
+
+
+Lemma tl_times_comm_aeq tl tl' :
+  tl_times tl tl' =tl= tl_times tl' tl.
+Proof.
+  rewrite 2 tl_times_spec_defn_correct.
+  destruct tl as [lsums labs], tl' as [rsums rabs].
+  cbn.
+  eexists; cbn -[reverse].
+  rewrite 2 reverse_app.
+  split; [|split; [apply ppermute_pbig_swap_app|]];
+  [eapply pbig_swap_posperm'; rewrite lengthN_app, 2 lengthN_reverse; lia|].
+  rewrite Permutation_app_comm.
+  rewrite fmap_app, <- 2 list_fmap_compose.
+  pose proof (lengthN_correct rsums).
+  pose proof (lengthN_correct lsums).
+  rewrite 2 lengthN_reverse, lengthN_app.
+  apply Permutation_app; apply eq_reflexivity, list_fmap_ext;
+    intros _ ((f, low), up) _; cbn;
+    rewrite <- 2 list_fmap_compose;
+    apply abs_fmap_l_ext; rewrite <- 2 fmap_app;
+    generalize (low ++ up); intros l;
+    apply list_fmap_ext;
+    (intros _ [r| |] _; [cbn|reflexivity..]);
+    unfold pbig_swap;
+    repeat case_decide; f_equal; lia || reflexivity.
+Qed.
+
+(* FIXME: Move *)
+(* Lemma Pmap_posperm_of *)
+
+Lemma map_inverses_empty `{FinMap A MA, FinMap B MB} :
+  map_inverses (∅ :> MA B) (∅ :> MB A).
+Proof.
+  intros ? ?.
+  rewrite 2 lookup_empty.
+  easy.
+Qed.
+
+(* FIXME: Move *)
+
+Definition tl_well_bound (tl : tensorlist) : Prop :=
+  abstracts_rel_vars tl.(tl_abstracts) ⊆
+  list_to_set (pseq 1 (lengthN tl.(tl_sums))).
+
+(* FIXME: Move*)
+Lemma relabel_abs_compose {A B C} (f : A -> B) (g : B -> C) l :
+  relabel_abs g (relabel_abs f l) = relabel_abs (g ∘ f) l.
+Proof.
+  unfold relabel_abs.
+  destruct l as ((idx, low), up).
+  now rewrite <- 2 list_fmap_compose.
+Qed.
+Lemma relabel_rels_id v : relabel_rels id v = v.
+Proof. now destruct v. Qed.
+Lemma relabel_rels_id' f v :
+  (forall r, f r = r) -> relabel_rels f v = v.
+Proof.
+  intros Hf.
+  erewrite relabel_rels_ext; [apply relabel_rels_id|apply Hf].
+Qed.
+
+
+Add Parametric Morphism : mk_tl with signature
+  eq ==> Permutation ==> tl_aeq as mk_tl_aeq_Permutation.
+Proof.
+  intros sums abs abs' Habs'.
+  exists id.
+  cbn.
+  split; [apply posperm_id|].
+  split; [apply ppermute_id|].
+  rewrite Habs'.
+  apply eq_reflexivity, symmetry, list_fmap_id'.
+  intros x _.
+  apply relabel_abs_id'.
+  intros v.
+  apply relabel_rels_id'.
+  intros; unfold make_pwf; case_decide; reflexivity.
+Qed.
+
+Add Parametric Morphism {A B} : fmap with signature
+  pointwise_relation A (@eq B) ==> (@eq (list A)) ==> (@eq (list B)) as list_fmap_mor.
+Proof.
+  intros; unfold pointwise_relation;
+  apply list_fmap_ext; auto.
+Qed.
+
+(* FIXME: Move!!!! *)
+#[global] Instance var_inhabited : Inhabited var := populate (rel 1).
+
+Lemma extend_match_of_abstract_tensors_correct'
+  (P : Pmap Idx -> Pmap Idx -> Pmap var -> Pset ->
+    list (Idx * list var * list var) -> Prop)
+  `{HP : forall mb mbi ml mlran rrest, Decision (P mb mbi ml mlran rrest)}
+  (labs rabs : list (Idx * list var * list var))
+  mb' mbi' ml' mlran' rrest :
+
+  extend_match_of_abstract_tensors P ∅ ∅ ∅ ∅ labs rabs =
+    Some (mb', mbi', ml', mlran', rrest) ->
+
+  P mb' mbi' ml' mlran' rrest /\
+  map_inverses mb' mbi' /\
+  dom mb' = abstracts_rel_vars labs /\
+  dom mbi' ⊆ abstracts_rel_vars rabs /\
+  map_img ml' ⊆ abstracts_vars rabs /\
+  set_Forall (λ r, mbi' !! r = None) mlran' /\
+  map_img (omap v2rel ml') = mlran' /\
+  dom ml' = abstracts_local_vars labs /\
+  (relabel_abs (var_elim (fmap rel ∘ (mb' !!.)) (ml' !!.)
+     (λ g, Some (glob g))) <$> labs) ++
+     (relabel_abs Some <$> rrest) ≡ₚ relabel_abs Some <$> rabs /\
+  (relabel_abs (var_elim (rel ∘ (mb' !!!.)) (ml' !!!.)
+     (glob)) <$> labs) ++
+     rrest ≡ₚ rabs /\
+  forall a,
+    a ∈ labs
+    → relabel_abs
+        (var_elim (fmap rel ∘ λ i : Idx, mb' !! i)
+           (λ i : Idx, ml' !! i) (λ g : Idx, Some (glob g))) a
+      ∈ relabel_abs Some <$> rabs.
+Proof.
+  intros Heq.
+  apply extend_match_of_abstract_tensors_correct in Heq;
+  [|apply map_inverses_empty|apply set_Forall_empty|reflexivity].
+  assert (Hsubs :
+    (relabel_abs
+     (var_elim (fmap rel ∘ λ i : Idx, mb' !! i)
+        (λ i : Idx, ml' !! i) (λ g : Idx, Some (glob g))) <$> labs) ⊆
+        relabel_abs Some <$> rabs). 1: {
+      intros x Hx.
+    rewrite <- Heq.2.2.2.2.2.2.2.2.2, elem_of_app; now left.
+    }
+  pose proof (fun x Hx => Hsubs _ (elem_of_list_fmap_1 _ labs x Hx)) as Hsubs'.
+  rewrite 2 dom_empty_L, 2 union_empty_l_L in Heq.
+  split_and!; [..|solve [auto]]; try apply Heq;
+  destruct Heq as (_ & _ & _ & _ & Hinvs & Hdom & Hdisjl & Himg & Hldom & Heq).
+  - intros q (p & Hp)%elem_of_dom.
+    apply Hinvs in Hp as Hp'.
+
+    (* pose proof (fun x => elem_of_Permutation_proper x _ _ Heq) as Heq'. *)
+    apply elem_of_dom_2 in Hp' as Hpdom.
+    rewrite Hdom in Hpdom.
+    set_unfold in Hpdom.
+    destruct Hpdom as (a & Hpa & Ha).
+    apply Hsubs' in Ha as Ha'.
+    apply elem_of_list_fmap in Ha' as (x & Hx & Hxrabs).
+    unfold abstracts_rel_vars.
+    apply elem_of_list_to_set, elem_of_list_bind.
+    exists x.
+    split; [|easy].
+    destruct a as ((idx, low), up), x as ((idx', low'), up').
+    cbn in Hx.
+    rewrite elem_of_list_omap.
+    exists (rel q).
+    split; [|reflexivity].
+    revert Hx.
+    intros [= <- Hl Hu].
+    rewrite elem_of_app.
+    apply elem_of_list_omap in Hpa
+      as ([] & [Hpl|Hpu]%elem_of_app & [= ->]).
+    + left.
+      apply elem_of_list_lookup in Hpl as (i & Hi).
+      apply (f_equal (.!! i)) in Hl.
+      rewrite 2 list_lookup_fmap, Hi in Hl.
+      cbn in Hl.
+      rewrite Hp' in Hl.
+      cbn in Hl.
+      apply elem_of_list_lookup.
+      exists i.
+      destruct (low' !! i); cbn in Hl; congruence.
+    + right.
+      apply elem_of_list_lookup in Hpu as (i & Hi).
+      apply (f_equal (.!! i)) in Hu.
+      rewrite 2 list_lookup_fmap, Hi in Hu.
+      cbn in Hu.
+      rewrite Hp' in Hu.
+      cbn in Hu.
+      apply elem_of_list_lookup.
+      exists i.
+      destruct (up' !! i); cbn in Hu; congruence.
+  - intros v (l & Hl)%elem_of_map_img.
+    apply elem_of_dom_2 in Hl as Hl'.
+    rewrite Hldom in Hl'.
+    apply elem_of_list_to_set, elem_of_list_bind in Hl' as (a & Hla & Ha).
+    apply Hsubs' in Ha.
+    apply elem_of_list_fmap in Ha as (b & Hab & Hb).
+    apply elem_of_list_to_set, elem_of_list_bind.
+    exists b.
+    split; [|easy].
+    destruct a as ((idx, low), up), b as ((idx', low'), up').
+    cbn in Hab.
+    revert Hab.
+    intros [= <- Hlow Hup].
+    apply elem_of_app.
+    apply elem_of_list_omap in Hla as
+      ([|_|] & [Hll|Hlu]%elem_of_app & [= ->]).
+    + left.
+      apply elem_of_list_lookup in Hll as (i & Hi).
+      apply (f_equal (.!! i)) in Hlow.
+      rewrite 2 list_lookup_fmap, Hi in Hlow.
+      cbn in Hlow.
+      apply elem_of_list_lookup.
+      exists i.
+      destruct (low' !! i); cbn in *; congruence.
+    + right.
+      apply elem_of_list_lookup in Hlu as (i & Hi).
+      apply (f_equal (.!! i)) in Hup.
+      rewrite 2 list_lookup_fmap, Hi in Hup.
+      cbn in Hup.
+      apply elem_of_list_lookup.
+      exists i.
+      destruct (up' !! i); cbn in *; congruence.
+  - apply (fmap_Permutation (relabel_abs (default (rel 1)))) in Heq
+      as Hdecomp'.
+    rewrite <- list_fmap_compose in Hdecomp'.
+    rewrite (list_fmap_id' (_ ∘ _)) in Hdecomp'. 2:{
+      intros abs _.
+      unfold compose.
+      rewrite relabel_abs_compose.
+      apply relabel_abs_id.
+    }
+    rewrite <- Hdecomp'.
+    rewrite fmap_app, <- 2 list_fmap_compose.
+    unfold compose at 1.
+    symmetry.
+    erewrite list_fmap_ext by now intros; apply relabel_abs_compose.
+    erewrite (list_fmap_ext (_ ∘ _)) by now
+      intros; unfold compose; rewrite relabel_abs_compose; apply relabel_abs_id.
+    rewrite list_fmap_id.
+    apply eq_reflexivity.
+    f_equal.
+    apply list_fmap_ext.
+    intros _ a _.
+    apply relabel_abs_ext.
+    intros [r|l|g]; [|reflexivity..].
+    cbn; rewrite lookup_total_alt.
+    destruct (_ !! _); reflexivity.
+Qed.
+
+Lemma map_inverses_comm `{Lookup A B MA, Lookup B A MB} (ma : MA) (mb : MB) :
+  map_inverses ma mb <-> map_inverses mb ma.
+Proof.
+  unfold map_inverses. firstorder.
+Qed.
+
+Lemma map_inverses_card_img `{FinMapDom A MA SA, !Elements A SA,
+  !FinSet A SA, FinMap B MB, FinSet B SB, !RelDecision (∈@{SB}) }
+  (ma : MA B) (mb : MB A) :
+  map_inverses ma mb ->
+  size (dom ma :> SA) = size (map_img ma :> SB).
+Proof.
+  intros Hinv.
+  rewrite map_dom_img_eq_card_iff_inj.
+  intros ? ? ? ?%Hinv ?%Hinv.
+  congruence.
+Qed.
+
+Lemma map_inverses_img `{FinMap A MA, FinMapDom B MB SB}
+  (ma : MA B) (mb : MB A) :
+    map_inverses ma mb ->
+    map_img ma ≡@{SB} dom mb.
+Proof.
+  intros Hab x.
+  rewrite elem_of_map_img, elem_of_dom.
+  setoid_rewrite (fun x => Hab x).
+  reflexivity.
+Qed.
+
+
+Lemma map_inverses_img_L `{FinMap A MA, FinMapDom B MB SB, !LeibnizEquiv SB}
+  (ma : MA B) (mb : MB A) :
+    map_inverses ma mb ->
+    map_img ma =@{SB} dom mb.
+Proof.
+  unfold_leibniz.
+  apply map_inverses_img.
+Qed.
+
+(* FIXME: Move *)
+Lemma and_from_l {P Q} :
+  P /\ (P -> Q) -> P /\ Q.
+Proof.
+  tauto.
+Qed.
+
+Definition tl_well_typed_aux tc sums abs :=
+  let tc' := tc_app_types (reverse sums) tc in
+  Forall (fun '(f, low, up) =>
+  fmap Some <$> tc_ma tc' !! f = Some (tc_get_var tc' <$> low ++ up)) abs.
+
+Notation tl_well_typed tc tl :=
+    (tl_well_typed_aux tc tl.(tl_sums) tl.(tl_abstracts)).
+
+Lemma well_typed_tproducts tc tes :
+  well_typed tc (tproducts tes) <-> Forall (well_typed tc) tes.
+Proof.
+  induction tes; [naive_solver|].
+  rewrite Forall_cons, <- IHtes.
+  cbn.
+  destruct tes; naive_solver.
+Qed.
+
+Lemma tl_well_typed_correct tc tl :
+  tl_well_typed tc tl <-> well_typed tc tl.
+Proof.
+  destruct tl as [sums abs].
+  cbn.
+  revert tc; induction sums; intros tc.
+  - cbn.
+    rewrite well_typed_tproducts.
+    unfold tl_well_typed_aux.
+    rewrite Forall_fmap.
+    apply Forall_iff.
+    intros ((f, low), up).
+    cbn.
+    now destruct tc.
+  - cbn.
+    rewrite <- IHsums.
+    unfold tl_well_typed_aux.
+    destruct tc; unfold tc_app_types; rewrite reverse_cons; cbn.
+    rewrite <- app_assoc.
+    reflexivity.
+Qed.
+
+(* FIXME: Move *)
+Lemma elem_of_abstracts_rel_vars l abs :
+  l ∈ abstracts_rel_vars abs <->
+  exists idx low up, (idx, low, up) ∈ abs /\ rel l ∈ low ++ up.
+Proof.
+  unfold abstracts_rel_vars.
+  rewrite elem_of_list_to_set, elem_of_list_bind.
+  rewrite 2 exists_pair.
+  setoid_rewrite elem_of_list_omap.
+  split; [|naive_solver].
+  intros (idx & low & up & ([] & ? & [= ->]) & ?).
+  eauto.
+Qed.
+Lemma elem_of_abstracts_local_vars l abs :
+  l ∈ abstracts_local_vars abs <->
+  exists idx low up, (idx, low, up) ∈ abs /\ loc l ∈ low ++ up.
+Proof.
+  unfold abstracts_local_vars.
+  rewrite elem_of_list_to_set, elem_of_list_bind.
+  rewrite 2 exists_pair.
+  setoid_rewrite elem_of_list_omap.
+  split; [|naive_solver].
+  intros (idx & low & up & ([] & ? & [= ->]) & ?).
+  eauto.
+Qed.
+Lemma elem_of_abstracts_global_vars l abs :
+  l ∈ abstracts_global_vars abs <->
+  exists idx low up, (idx, low, up) ∈ abs /\ glob l ∈ low ++ up.
+Proof.
+  unfold abstracts_global_vars.
+  rewrite elem_of_list_to_set, elem_of_list_bind.
+  rewrite 2 exists_pair.
+  setoid_rewrite elem_of_list_omap.
+  split; [|naive_solver].
+  intros (idx & low & up & ([] & ? & [= ->]) & ?).
+  eauto.
+Qed.
+
+
+Lemma extend_match_of_abstract_tensors_correct_WT_pre
+  (P : Pmap Idx -> Pmap Idx -> Pmap var -> Pset ->
+    list (Idx * list var * list var) -> Prop)
+  `{HP : forall mb mbi ml mlran rrest, Decision (P mb mbi ml mlran rrest)}
+  (labs rabs : list (Idx * list var * list var))
+  mb' mbi' ml' mlran' rrest :
+
+  extend_match_of_abstract_tensors P ∅ ∅ ∅ ∅ labs rabs =
+    Some (mb', mbi', ml', mlran', rrest) ->
+  forall tc univ lsums rsums,
+  tl_well_typed_aux (tc_eqn_with_locals tc univ) lsums labs ->
+  tl_well_typed_aux tc rsums rabs ->
+  (forall l ty v, univ !! l = Some ty -> ml' !! l = Some v ->
+    tc_get_var (tc_app_types (reverse rsums) tc) v = Some ty) /\
+  (forall (r r' : Idx) ty, reverse lsums !! (r:>nat) = Some ty ->
+    mb' !! r = Some r' -> (reverse rsums ++ tc.(tc_mr)) !! (r':>nat) = Some ty).
+Proof.
+  intros Hext tc univ lsums rsums Hl Hr.
+  apply extend_match_of_abstract_tensors_correct' in Hext as
+    (_ & Hinvs & Hdom_mb & Hdom_mbi & Hlimg & Hldisj & Hmlran
+      & Hdomml & Hpermeq & Hperm & Hsubs).
+  split.
+  - intros l ty v Hty_univ Hml'_v.
+    apply elem_of_dom_2 in Hml'_v as Hv.
+    rewrite Hdomml in Hv.
+    apply elem_of_abstracts_local_vars in Hv as (idx & low & up & Hinl & Hl_lu).
+    apply Hsubs in Hinl as Hlu_r.
+    cbn in Hlu_r.
+    apply elem_of_list_fmap in Hlu_r as (((idx', low'), up') & Heq & Hinr).
+    cbn in Heq.
+    revert Heq.
+    intros [= <- Hlow Hup].
+    hnf in Hr, Hl.
+    rewrite Forall_forall in Hr, Hl.
+    specialize (Hr _ Hinr).
+    specialize (Hl _ Hinl).
+    cbn in Hr, Hl.
+    generalize (f_equal2 app Hlow Hup).
+    rewrite <- 2 fmap_app.
+    intros Hlowup.
+    remember (low ++ up) as lowup eqn:Hlowup_eq.
+    remember (low' ++ up') as lowup' eqn:Hlowup'_eq.
+    apply elem_of_list_lookup in Hl_lu as (i & Hi).
+    apply (f_equal (.!! i)) in Hlowup.
+    rewrite 2 list_lookup_fmap, Hi in Hlowup.
+    cbn in Hlowup.
+    rewrite Hml'_v in Hlowup.
+    destruct (lowup' !! i) as [?|] eqn:Hlowup'_i; [|easy].
+    cbn in Hlowup.
+    revert Hlowup.
+    intros [= <-].
+    apply (f_equal (λ ml, (.!! i) <$> ml)) in Hl, Hr.
+    cbn in Hl, Hr.
+    rewrite Hl in Hr.
+    rewrite 2 list_lookup_fmap in Hr.
+    rewrite Hi, Hlowup'_i in Hr.
+    cbn in Hr.
+    injection Hr.
+    intros <-.
+    rewrite lookup_union, Hty_univ.
+    now rewrite union_Some_l.
+  - intros r r' ty Hl_r Hmb_r.
+    apply elem_of_dom_2 in Hmb_r as Hrdom.
+    rewrite Hdom_mb in Hrdom.
+    apply elem_of_abstracts_rel_vars in Hrdom as (idx & low & up & Hinl & Hl_lu).
+    apply Hsubs in Hinl as Hlu_r.
+    cbn in Hlu_r.
+    apply elem_of_list_fmap in Hlu_r as (((idx', low'), up') & Heq & Hinr).
+    cbn in Heq.
+    revert Heq.
+    intros [= <- Hlow Hup].
+    hnf in Hr, Hl.
+    rewrite Forall_forall in Hr, Hl.
+    specialize (Hr _ Hinr).
+    specialize (Hl _ Hinl).
+    cbn in Hr, Hl.
+    generalize (f_equal2 app Hlow Hup).
+    rewrite <- 2 fmap_app.
+    intros Hlowup.
+    remember (low ++ up) as lowup eqn:Hlowup_eq.
+    remember (low' ++ up') as lowup' eqn:Hlowup'_eq.
+    apply elem_of_list_lookup in Hl_lu as (i & Hi).
+    apply (f_equal (.!! i)) in Hlowup.
+    rewrite 2 list_lookup_fmap, Hi in Hlowup.
+    cbn in Hlowup.
+    rewrite Hmb_r in Hlowup.
+    destruct (lowup' !! i) as [?|] eqn:Hlowup'_i; [|easy].
+    cbn in Hlowup.
+    revert Hlowup.
+    intros [= <-].
+    apply (f_equal (λ ml, (.!! i) <$> ml)) in Hl, Hr.
+    cbn in Hl, Hr.
+    rewrite Hl in Hr.
+    rewrite 2 list_lookup_fmap in Hr.
+    rewrite Hi, Hlowup'_i in Hr.
+    cbn in Hr.
+    injection Hr.
+    rewrite app_nil_r.
+    intros <-.
+    easy.
+Qed.
+
+Lemma tl_well_typed_well_bound mabs mg ml tl :
+  tl_well_typed (mk_tc mabs mg ml []) tl ->
+  tl_well_bound tl.
+Proof.
+  intros HWT.
+  hnf in HWT |- *.
+  intros r (idx & low & up & Hlu_in & Hin_lu)%elem_of_abstracts_rel_vars.
+  rewrite Forall_forall in HWT.
+  specialize (HWT _ Hlu_in).
+  cbn in HWT.
+  apply elem_of_list_lookup in Hin_lu as (i & Hi).
+  apply (f_equal (λ ml, (.!! i) <$> ml)) in HWT.
+  revert HWT.
+  cbn.
+  destruct (mabs !! idx) as [tys|]; [|easy].
+  cbn.
+  rewrite 2 list_lookup_fmap, Hi.
+  cbn.
+  rewrite app_nil_r.
+  destruct (tys !! i) as [tyi|]; [|easy].
+  cbn.
+  intros [= Heq%eq_sym%lookup_lt_Some].
+  rewrite length_reverse in Heq.
+  rewrite lengthN_correct_rev, elem_of_list_to_set, elem_of_pseq_1.
+  lia.
+Qed.
+
+
+
+Lemma tl_well_typed_aux_mono mabs mg ml mabs' mg' ml' mr sums abs :
+  mabs ⊆ mabs' -> mg ⊆ mg' -> ml ⊆ ml' ->
+  tl_well_typed_aux (mk_tc mabs mg ml mr) sums abs ->
+  tl_well_typed_aux (mk_tc mabs' mg' ml' mr) sums abs.
+Proof.
+  intros Habs Hg Hl.
+  intros Hall.
+  eapply Forall_impl; [exact Hall|].
+  intros ((f, low), up).
+  cbn.
+  destruct (mabs !! f) as [mf|] eqn:Hmf; [|easy].
+  eapply lookup_weaken in Hmf as Hm'f; [|eassumption].
+  rewrite Hm'f.
+  cbn.
+  intros [= HSmf].
+  f_equal.
+  apply (list_eq_same_length _ _ _ eq_refl);
+    [apply (f_equal length) in HSmf; now rewrite ?length_fmap in *|].
+  rewrite length_fmap.
+  intros i x y Hi.
+  rewrite 2 list_lookup_fmap.
+  destruct (mf !! i) as [mfi|] eqn:Hmfi; [|easy].
+  cbn.
+  intros [= <-].
+  apply (f_equal (.!! i)) in HSmf.
+  rewrite 2 list_lookup_fmap, Hmfi in HSmf.
+  cbn in HSmf.
+  destruct ((low ++ up) !! i) as [v|] eqn:Hv; [cbn|easy].
+  intros [= <-].
+  cbn in HSmf.
+  revert HSmf.
+  intros [= Heq].
+  destruct v as [r|l|g]; cbn in *;
+  [easy|symmetry in Heq |- *; eapply lookup_weaken; eassumption..].
+Qed.
+
+
+
+Lemma pos_to_nat_pred_of_nat (i : nat) :
+  pos_to_nat_pred (Pos.of_succ_nat i) = i.
+Proof.
+  lia.
+Qed.
+
+Lemma lookup_list_to_map_imap_to_pos `{FinMap positive M} {A B}
+  (f : A -> B) (l : list A) (i : positive) :
+  (list_to_map (imap (fun j v => (Pos.of_succ_nat j, f v)) l) :> M B) !! i =
+  f <$> (l !! (i:>nat)).
+Proof.
+  apply option_eq.
+  intros x.
+  rewrite <- elem_of_list_to_map. 2:{
+    rewrite fmap_imap.
+    unfold compose.
+    cbn.
+    rewrite imap_seq_0.
+    apply NoDup_fmap_2; [hnf; lia|].
+    apply NoDup_seq.
+  }
+  rewrite elem_of_lookup_imap.
+  split.
+  - intros (i' & z & [= -> ->] & Heq).
+    now rewrite pos_to_nat_pred_of_nat, Heq.
+  - destruct (l !! (i:>nat)) as [li|] eqn:Heq; [|easy].
+    cbn.
+    intros [= <-].
+    exists (i:>nat).
+    rewrite pos_to_nat_pred_to_pos.
+    eauto.
+Qed.
+
+Lemma relabel_abs_ext_strong {A B} (f g : A -> B) abs :
+  (forall x, x ∈ abs.1.2 ++ abs.2 ->
+    f x = g x) -> relabel_abs f abs = relabel_abs g abs.
+Proof.
+  intros Hfg.
+  unfold relabel_abs.
+  destruct abs as ((idx, low), up).
+  f_equal; [f_equal|]; apply list_fmap_ext; intros _ ? ?%elem_of_list_lookup_2;
+  apply Hfg, elem_of_app; [left|right]; easy.
+Qed.
+
+Lemma relabel_abs_id_strong {A} (f : A -> A) abs :
+  (forall x, x ∈ abs.1.2 ++ abs.2 -> f x = x) -> relabel_abs f abs = abs.
+Proof.
+  intros Hf.
+  transitivity (relabel_abs id abs); [|apply relabel_abs_id].
+  now apply relabel_abs_ext_strong.
+Qed.
+
+Lemma relabel_rels_compose g f v :
+  relabel_rels g (relabel_rels f v) =
+  relabel_rels (g ∘ f) v.
+Proof.
+  now destruct v.
+Qed.
+
+Lemma imap_to_fmap {A B} (f : A -> B) l :
+  imap (fun _ => f) l = f <$> l.
+Proof.
+  induction l; cbn; rewrite <- ? IHl; reflexivity.
+Qed.
+
+Lemma elem_of_abstracts_vars v abs :
+  v ∈ abstracts_vars abs <-> exists idx low up,
+    (idx, low, up) ∈ abs /\ v ∈ low ++ up.
+Proof.
+  set_unfold.
+  rewrite 2 exists_pair.
+  setoid_rewrite elem_of_app.
+  firstorder.
+Qed.
+
+Lemma elem_of_abstracts_vars_rel r abs :
+  rel r ∈ abstracts_vars abs <-> r ∈ abstracts_rel_vars abs.
+Proof.
+  now rewrite elem_of_abstracts_rel_vars, elem_of_abstracts_vars.
+Qed.
+
+Lemma elem_of_abstracts_vars_loc r abs :
+  loc r ∈ abstracts_vars abs <-> r ∈ abstracts_local_vars abs.
+Proof.
+  now rewrite elem_of_abstracts_local_vars, elem_of_abstracts_vars.
+Qed.
+
+Lemma elem_of_abstracts_vars_glob r abs :
+  glob r ∈ abstracts_vars abs <-> r ∈ abstracts_global_vars abs.
+Proof.
+  now rewrite elem_of_abstracts_global_vars, elem_of_abstracts_vars.
+Qed.
+
+Lemma and_exists_l {A} {P Q} : (P /\ exists a : A, Q a) <-> 
+  exists a, P /\ Q a.
+Proof.
+  firstorder.
+Qed.
+
+
+Lemma match_tensorlist_aux_correct mabs mg univ univ' lhs targ utl relmap locmap :
+  match_tensorlist_aux lhs targ = Some (utl, relmap, locmap) ->
+  all_bound lhs ->
+  tl_well_typed (mk_tc mabs mg univ []) lhs ->
+  tl_well_typed (mk_tc mabs mg univ' []) targ ->
+  (* tl_well_bound targ -> *)
+  abstracts_local_vars lhs.(tl_abstracts) = dom locmap /\
+  (forall l ty v, univ !! l = Some ty -> locmap !! l = Some v ->
+    tc_get_var (mk_tc mabs mg univ' (reverse utl.(tl_sums))) v = Some ty) /\
+  targ =tl= fill_tensorlist_rewrite utl lhs relmap locmap.
+Proof.
+  cbv delta [match_tensorlist_aux] beta.
+  destruct (extend_match_of_abstract_tensors _ _ _ _ _ _ _)
+    as [((((mb, mbi), ml), mlran), rrest)|] eqn:Hext; [|intros [=]].
+  pose proof Hext as Hext'.
+  intros Heq.
+  apply (inj Some) in Heq.
+  revert Heq.
+  cbv zeta.
+  set (ntys := imap _ (reverse _)).
+  set (unused_tys := filter _ ntys).
+  set (newty_info := imap _ unused_tys).
+  set (rrest_map := list_to_map _).
+  set (newtys := reverse _).
+  set (ml' := relabel_rels _ <$> ml).
+  intros [= <- <- <-].
+  intros Hlhs Htylhs Htytarg.
+  apply tl_well_typed_well_bound in Htytarg as Htarg.
+
+  apply extend_match_of_abstract_tensors_correct' in Hext as
+    (Hrestdisj & Hinvs & Hdom & Hdommbi & Hlimg & Hldisj & Hmlran &
+      Hldom & Hdecomp & Hperm & Hsubs).
+  destruct targ as [tsums tabs], lhs as [rsums rabs].
+  unfold all_bound, tl_well_bound in Hlhs, Htarg.
+  cbn [tl_sums tl_abstracts] in *.
+  split. 1:{
+    unfold ml'.
+    rewrite dom_fmap_L.
+    auto.
+  }
+
+  assert (Hlenlt : (length rsums <= length tsums)%nat). 1:{
+    apply (map_inverses_card_img (SB:=Pset)) in Hinvs as Hcard.
+    rewrite Hdom in Hcard.
+    rewrite Hlhs in Hcard.
+    rewrite size_list_to_set, length_pseq, lengthN_correct
+      in Hcard by apply NoDup_pseq.
+    rewrite map_inverses_img in Hcard by eassumption.
+    rewrite Hcard.
+    eapply Nat.le_trans;
+    [apply subseteq_size, Hdommbi|].
+    rewrite <- lengthN_correct, <- (length_pseq 1),
+      <- (size_list_to_set (C:=Pset))
+      by apply NoDup_pseq.
+    apply subseteq_size.
+    apply Htarg.
+  }
+
+  assert (Hdommbi' : dom mbi =
+    list_to_set (filter (λ '(idx, _), is_Some (mbi !! idx)) ntys).*1). 1:{
+
+    setoid_rewrite <- leibniz_equiv_iff.
+    intros x.
+    rewrite elem_of_dom.
+    rewrite elem_of_list_to_set, elem_of_list_fmap.
+    setoid_rewrite elem_of_list_filter.
+    unfold ntys.
+    setoid_rewrite elem_of_lookup_imap.
+    split; cycle 1.
+    + intros ([] & -> & Hsome & _).
+      apply Hsome.
+    + intros Hx.
+      rewrite Htarg in Hdommbi.
+      specialize (Hdommbi x ltac:(now apply elem_of_dom))
+        as Hxlt%elem_of_list_to_set%elem_of_pseq_1.
+      specialize (lookup_lt_is_Some (reverse tsums) x).2 as Hlx.
+      tspecialize Hlx by now rewrite length_reverse, <- lengthN_correct; lia.
+      destruct Hlx as [rx Hrx].
+      exists (x, rx).
+      split; [easy|].
+      split; [easy|].
+      exists x, rx.
+      split; [f_equal; lia|].
+      apply Hrx.
+  }
+
+  assert (HNoDup_fsts_filter :
+    NoDup (filter (λ '(idx, _), is_Some (mbi !! idx)) ntys).*1). 1:{
+
+    eapply (fun H => ((NoDup_app _ _).1 H).1).
+    rewrite <- fmap_app.
+    rewrite filter_with_neg_Permutation.
+    unfold ntys.
+    rewrite fmap_imap.
+    unfold compose.
+    cbn.
+    rewrite imap_seq_0.
+    apply NoDup_fmap_2; [hnf; clear; lia|].
+    apply NoDup_seq.
+  }
+
+  assert (HNoDup_fsts_filter' :
+    NoDup (filter (λ '(idx, _), ¬ is_Some (mbi !! idx)) ntys).*1). 1:{
+
+    eapply (fun H => ((NoDup_app _ _).1 H).1).
+    rewrite <- fmap_app.
+    rewrite filter_with_neg_Permutation.
+    unfold ntys.
+    rewrite fmap_imap.
+    unfold compose.
+    cbn.
+    rewrite imap_seq_0.
+    apply NoDup_fmap_2; [hnf; clear; lia|].
+    apply NoDup_seq.
+  }
+
+  assert (Hlens : (length rsums + length unused_tys = length tsums)%nat). 1:{
+    transitivity (length ntys);
+    [|subst ntys; now rewrite length_imap, length_reverse].
+
+    erewrite <- (filter_neg_with_Permutation (P:=λ '(idx, _), is_Some (mbi !! idx)) ntys).
+    rewrite length_app, Nat.add_comm.
+    f_equal; [f_equal; apply list_filter_iff; now intros []|].
+
+    apply (map_inverses_card_img (SB:=Pset)) in Hinvs as Hcard.
+    rewrite Hdom in Hcard.
+    rewrite Hlhs in Hcard.
+    rewrite size_list_to_set, length_pseq, lengthN_correct
+      in Hcard by apply NoDup_pseq.
+    rewrite map_inverses_img in Hcard by eassumption.
+    rewrite Hcard.
+    rewrite <- (length_fmap fst).
+    rewrite <- (size_list_to_set (C:=Pset)) by easy.
+    f_equal.
+    assumption.
+  }
+
+  rewrite <- Hperm.
+
+  cbv delta [fill_tensorlist_rewrite] beta match zeta.
+  set (shift := relabel_rels _).
+  rewrite Permutation_app_comm.
+
+
+  assert (Hnewty_info_alt :
+    newty_info = imap (λ inew iold_ty,
+      (iold_ty.1, Pos.of_succ_nat inew, iold_ty.2)) unused_tys). 1:{
+    apply imap_ext; now intros ? [].
+  }
+
+  assert (HNoDup_newty_info_1_1 : NoDup newty_info.*1.*1). 1:{
+    rewrite Hnewty_info_alt.
+    rewrite 2 fmap_imap.
+    unfold compose; cbn.
+    rewrite imap_to_fmap.
+    unfold unused_tys.
+    apply HNoDup_fsts_filter'.
+  }
+
+
+  set (used_tys := filter (λ '(idx, _), is_Some (mbi !! idx)) ntys).
+  set (oldty_info := imap (λ inew '(iold, ty), (iold, Pos.of_succ_nat inew, ty))
+    used_tys).
+  set (rrest_inv_map := list_to_map (prod_swap <$> newty_info.*1) :> Pmap Idx).
+
+
+  pose proof (lengthN_correct tsums).
+  pose proof (lengthN_correct rsums).
+  pose proof (lengthN_correct unused_tys).
+
+  assert (Hrrest_inv_inv : forall x, x ∈ abstracts_rel_vars tabs ->
+    ¬ (is_Some (mbi !! x)) ->
+    (if decide (Pmap_map rrest_map x < lengthP unused_tys)
+    then rrest_inv_map !!! Pmap_map rrest_map x
+    else pos_add_N (Pmap_map rrest_map x) (lengthN rsums)) = x). 1:{
+      clear Hrestdisj.
+      intros x Hx_rrest Hrestdisj.
+      assert (Hxdom : x ∈ dom rrest_map). 1:{
+        unfold rrest_map.
+        rewrite dom_list_to_map_L, elem_of_list_to_set.
+        unfold newty_info.
+        rewrite 2 fmap_imap.
+        unfold compose.
+        rewrite (imap_ext _ (λ _ x, x.1)) by now intros ? [].
+        rewrite imap_to_fmap.
+        unfold unused_tys.
+        rewrite elem_of_list_fmap.
+        cbn in Hrestdisj.
+        assert (Hxtys : ((x :> nat) < length tsums)%nat). 1:{
+          apply Htarg, elem_of_list_to_set, elem_of_pseq_1 in Hx_rrest; lia.
+        }
+        rewrite <- length_reverse in Hxtys.
+        apply lookup_lt_is_Some in Hxtys as Htx.
+        destruct Htx as [tx Htx].
+        exists (x, tx).
+        split; [reflexivity|].
+        apply elem_of_list_filter.
+        split; [easy|].
+        unfold ntys.
+        apply elem_of_lookup_imap.
+        exists x, tx.
+        split; [f_equal; lia|].
+        easy.
+      }
+      apply elem_of_dom in Hxdom as [rx Hrx].
+      unfold Pmap_map.
+      rewrite Hrx; cbn.
+      rewrite decide_True. 2:{
+        unfold rrest_map in Hrx.
+        rewrite <- elem_of_list_to_map in Hrx by easy.
+        apply elem_of_list_fmap in Hrx as ((? & ty) & Hsubst & Hin_newty_info).
+        cbn in Hsubst.
+        revert Hsubst.
+        intros <-.
+        rewrite Hnewty_info_alt in Hin_newty_info.
+        apply elem_of_lookup_imap in Hin_newty_info as (idx & [] & [= <- Hidxeq <-] & Hidx).
+        apply lookup_lt_Some in Hidx.
+        lia.
+      }
+      apply lookup_total_correct.
+      apply elem_of_list_to_map. 1:{
+        rewrite fsts_prod_swap.
+        rewrite Hnewty_info_alt.
+        rewrite 2 fmap_imap.
+        unfold compose.
+        cbn.
+        rewrite imap_seq_0.
+        apply NoDup_fmap_2; [hnf; lia|].
+        apply NoDup_seq.
+      }
+      rewrite elem_of_list_fmap.
+      exists (x, rx).
+      split; [reflexivity|].
+      unfold rrest_map in Hrx.
+      rewrite <- elem_of_list_to_map in Hrx by easy.
+      easy.
+  }
+
+  pose proof (extend_match_of_abstract_tensors_correct_WT_pre
+    _ _ _ _ _ _ _ _ Hext') as HWT.
+  specialize (HWT (mk_tc mabs mg univ' []) univ rsums tsums).
+  unfold tc_eqn_with_locals in HWT.
+  cbn in HWT.
+
+  specialize (fun H => HWT H Htytarg).
+  tspecialize HWT. 1:{
+    eapply tl_well_typed_aux_mono; try eassumption; [reflexivity..|].
+    apply map_union_subseteq_l.
+  }
+  rewrite (unfold tc_app_types), 2 app_nil_r in HWT.
+  cbn in HWT.
+  split. 1:{
+    unfold ml'.
+    intros l ty v Huniv_l.
+    rewrite lookup_fmap.
+    destruct (ml !! l) as [[r| |]|] eqn:Hml_l; [|
+    cbn; intros [= <-];
+    apply (HWT.1 l ty _ Huniv_l Hml_l)..|easy].
+    cbn.
+    intros [= <-].
+    cbn.
+    unfold newtys.
+    rewrite reverse_involutive.
+    rewrite list_lookup_fmap.
+    assert (Hrran : r ∈ mlran). 1:{
+      subst mlran.
+      rewrite elem_of_map_img.
+      exists l.
+      rewrite lookup_omap, Hml_l.
+      reflexivity.
+    }
+    assert (Hrdom : r ∈ dom (rrest_map)). 1:{
+      unfold rrest_map.
+      rewrite dom_list_to_map, elem_of_list_to_set.
+      rewrite Hnewty_info_alt.
+      rewrite 2 fmap_imap.
+      unfold compose.
+      cbn.
+      rewrite imap_to_fmap.
+      unfold unused_tys.
+      rewrite elem_of_list_fmap.
+      assert (Hnmbi : ¬ is_Some (mbi !! r)) by now rewrite Hldisj.
+      assert (Hrlt : ((r:>nat) < length tsums)%nat). 1:{
+        specialize (Hlimg (rel r)) as Hrvar.
+        tspecialize Hrvar by now apply elem_of_map_img; eauto.
+        rewrite elem_of_abstracts_vars_rel in Hrvar.
+        apply Htarg in Hrvar.
+        rewrite elem_of_list_to_set, elem_of_pseq_1 in Hrvar.
+        lia.
+      }
+      rewrite <- length_reverse in Hrlt.
+      apply lookup_lt_is_Some in Hrlt as Hlook.
+      destruct Hlook as [rtr Hrtr].
+      exists (r, rtr).
+      split; [easy|].
+      rewrite elem_of_list_filter.
+      split; [easy|].
+      apply elem_of_lookup_imap.
+      exists r, rtr.
+      split; [f_equal; lia|].
+      easy.
+    }
+    apply elem_of_dom in Hrdom as Hrr.
+    destruct Hrr as [rr_r Hrr_r].
+    unfold Pmap_map.
+    rewrite Hrr_r.
+    cbn.
+    (* unfold newty_info.
+    rewrite list_lookup_imap.
+    unfold unused_tys.
+    unfold rrest_map in Hrr_r. *)
+    apply elem_of_list_to_map in Hrr_r; [|easy].
+    apply elem_of_list_fmap in Hrr_r as (((_, _), ty') & [= <- <-] & Hin_nti).
+    rewrite Hnewty_info_alt in Hin_nti |- *.
+    rewrite elem_of_lookup_imap in Hin_nti.
+    destruct Hin_nti as (idx & (_, _) & [= <- -> <-] & Hlook).
+    rewrite list_lookup_imap.
+    rewrite pos_to_nat_pred_of_nat.
+    rewrite Hlook.
+    cbn.
+    specialize (HWT.1 l ty (rel r) Huniv_l Hml_l) as HWT'.
+    cbn in HWT'.
+    unfold unused_tys in Hlook.
+    apply elem_of_list_lookup_2 in Hlook as 
+      (Hnsome & (i & _ & [= -> <-] & Hlook)%elem_of_lookup_imap)%elem_of_list_filter.
+    rewrite pos_to_nat_pred_of_nat in *.
+    congruence.
+  }
+
+  
+  
+
+
+  (* exists (λ p, default _ (mbi) ) *)
+  (* symmetry. *)
+  exists (λ p, if decide (p < lengthP rsums) then
+    mb !!! p
+      else rrest_inv_map !!! (pos_sub_N p (lengthN rsums))).
+  cbn [tl_sums tl_abstracts] in *.
+
+
+
+  apply and_from_l, conj; [|intros Hpperm; apply and_from_l, conj;
+    [|intros Hppermute]].
+  - apply surj_is_posperm.
+    intros p Hp.
+    destruct_decide (decide (is_Some (mbi !! p))) as Hpbnd.
+    + destruct Hpbnd as [q Hq].
+      exists q.
+      apply Hinvs in Hq as Hq'.
+      apply elem_of_dom_2 in Hq' as Hqdom.
+      rewrite Hdom, Hlhs, elem_of_list_to_set, elem_of_pseq_1 in Hqdom.
+      split; [lia|].
+      rewrite decide_True by easy.
+      now apply lookup_total_correct.
+    + assert (Hunu : (p, (reverse tsums) !!! (p:>nat)) ∈ unused_tys). 1:{
+        apply elem_of_list_filter.
+        split; [easy|].
+        apply elem_of_list_lookup.
+        exists p.
+        unfold ntys.
+        rewrite list_lookup_imap.
+        pose proof (lookup_lt_is_Some (reverse tsums) p).2 as Hsome.
+        tspecialize Hsome by now rewrite length_reverse; lia.
+        rewrite list_lookup_total_alt.
+        destruct Hsome as [? ->].
+        cbn.
+        do 2 f_equal; lia.
+      }
+      apply elem_of_list_lookup in Hunu as (i & Hi).
+      exists (pos_add_N (Pos.of_succ_nat i) (lengthN rsums))%nat.
+      rewrite decide_False by lia.
+      replace (pos_sub_N _ _) with (Pos.of_succ_nat i) by lia.
+      unfold rrest_inv_map.
+      split; [apply lookup_lt_Some in Hi;
+      pose proof (lengthN_correct unused_tys); lia|].
+      apply lookup_total_correct.
+      apply elem_of_list_to_map.
+      * rewrite fsts_prod_swap.
+        unfold newty_info.
+        rewrite imap_to_zip_with_seq.
+        rewrite 2 fmap_zip_with.
+        replace (zip_with _ _ _) with (pseq 1 (lengthN unused_tys));
+          [apply NoDup_pseq|].
+        apply (fun H => list_eq_same_length _ _ _ H eq_refl);
+          [rewrite length_zip_with, length_pseq, lengthN_correct, length_seq;
+            apply Nat.min_id|].
+        rewrite length_pseq, lengthN_correct.
+        pose proof (lengthN_correct unused_tys).
+        intros j x y Hj.
+        rewrite lookup_pseq_1_lt by lia.
+        intros [= <-].
+        rewrite lookup_zip_with, lookup_seq_lt by lia.
+        cbn.
+        destruct (unused_tys !! j) as [[]|]; [|easy].
+        cbn.
+        now intros [= <-].
+      * rewrite elem_of_list_fmap.
+        exists (p, Pos.of_succ_nat i).
+        split; [reflexivity|].
+        apply elem_of_list_lookup.
+        exists i.
+        rewrite list_lookup_fmap.
+        unfold newty_info.
+        rewrite list_lookup_imap, Hi.
+        reflexivity.
+  - apply (fun H => list_eq_same_length _ _ _ H eq_refl);
+    rewrite length_ppermute. 1:{
+      rewrite 2 length_reverse, length_app.
+      rewrite <- Hlens, Nat.add_comm.
+      f_equal.
+      unfold newtys, newty_info.
+      now rewrite length_reverse, length_fmap, length_imap.
+    }
+    intros i x y Hi.
+    rewrite lookup_ppermute_alt_bdd by
+      (easy + apply posperm_bounded; now rewrite lengthN_reverse).
+    rewrite reverse_app.
+    case_decide as Hsmall.
+    + rewrite lookup_app_l by now rewrite length_reverse; lia.
+      assert (Hidom : Pos.of_succ_nat i ∈ dom mb). 1:{
+        rewrite Hdom, Hlhs, elem_of_list_to_set, elem_of_pseq_1; lia.
+      }
+      apply elem_of_dom in Hidom as [mb_i Hmb_i].
+      rewrite lookup_total_alt, Hmb_i.
+      cbn.
+      intros Ht_mb_i Hr_i.
+      specialize (HWT.2 (Pos.of_succ_nat i) mb_i y) as Heq.
+      rewrite pos_to_nat_pred_of_nat in Heq.
+      specialize (Heq Hr_i Hmb_i).
+      congruence.
+    + rewrite lookup_app_r by now rewrite !length_reverse; lia.
+      rewrite length_reverse.
+      unfold rrest_inv_map.
+      unfold newtys.
+      rewrite reverse_involutive.
+      unfold newty_info at 1.
+      rewrite 2 fmap_imap.
+      unfold compose; cbn.
+      erewrite (imap_ext _ (λ inew iold_ty,
+        (Pos.of_succ_nat inew, iold_ty.1))). 2:{
+        intros ? []; reflexivity.
+      }
+      rewrite lookup_total_alt.
+      rewrite lookup_list_to_map_imap_to_pos.
+      replace (pos_to_nat_pred (pos_sub_N _ _)) with (i - length rsums)%nat by lia.
+      unfold newty_info.
+      rewrite list_lookup_fmap.
+      rewrite list_lookup_imap.
+      destruct (unused_tys !! _) as [[iold ity]|] eqn:Heq; [|easy].
+      cbn.
+      unfold unused_tys in Heq.
+      apply elem_of_list_lookup_2 in Heq as [Hnmbi Helem]%elem_of_list_filter.
+      unfold ntys in Helem.
+      apply elem_of_lookup_imap in Helem as (iold' & ity' & [= -> <-] & Hlook).
+      rewrite pos_to_nat_pred_of_nat.
+      congruence.
+  - rewrite fmap_app.
+    apply Permutation_app.
+    + symmetry.
+      rewrite <- 2 list_fmap_compose.
+      apply eq_reflexivity.
+      apply list_fmap_id'.
+      intros ((f, low), up) Hlu_rrest.
+      unfold compose.
+      rewrite 2 relabel_abs_compose.
+      apply relabel_abs_id_strong.
+      intros x Hx.
+      cbn in Hx.
+      unfold compose.
+      unfold shift.
+      rewrite 2 relabel_rels_compose.
+      destruct x as [x| |]; [|reflexivity..].
+      cbn.
+      f_equal.
+      rewrite (decide_False (mb !!! _)) by lia.
+      rewrite <- decide_not, (decide_ext _ (Pmap_map rrest_map x < lengthP unused_tys))
+        by lia.
+      replace (pos_sub_N _ _) with (Pmap_map rrest_map x) by lia.
+
+      move Hrestdisj at bottom.
+      specialize (Hrestdisj x).
+      assert (Hx_rrest : x ∈ abstracts_rel_vars rrest) by
+        now rewrite elem_of_abstracts_rel_vars; eauto.
+      tspecialize Hrestdisj by auto.
+      apply Hrrest_inv_inv; [|easy].
+      enough (abstracts_rel_vars rrest ⊆ abstracts_rel_vars tabs) as Hsub
+        by now apply Hsub in Hx_rrest.
+      intros a.
+      rewrite 2 elem_of_abstracts_rel_vars.
+      enough (rrest ⊆ tabs) as Hsub by (clear -Hsub; naive_solver).
+      intros flu.
+      rewrite <- Hperm.
+      rewrite elem_of_app.
+      now right.
+    + rewrite <- list_fmap_compose.
+      apply eq_reflexivity.
+      apply list_fmap_ext.
+      intros _ ((f, low), up) Hflu%elem_of_list_lookup_2.
+      unfold compose.
+      rewrite relabel_abs_compose.
+      apply relabel_abs_ext_strong.
+      intros x Hx.
+      cbn in Hx.
+      cbn.
+      destruct x as [r|l|g]; cbn; [..|reflexivity].
+      * assert (Hrdom : r ∈ dom mb). 1:{
+          rewrite Hdom, elem_of_abstracts_rel_vars; eauto.
+        }
+        rewrite lookup_total_alt.
+        apply elem_of_dom in Hrdom as [mr Hmr].
+        rewrite Hmr.
+        cbn.
+        f_equal.
+        assert (Hrrel : r ∈ abstracts_rel_vars rabs) by
+          now rewrite elem_of_abstracts_rel_vars; eauto.
+        rewrite Hlhs, elem_of_list_to_set, elem_of_pseq_1 in Hrrel.
+        rewrite decide_False by lia.
+        rewrite decide_True by lia.
+        reflexivity.
+      * assert (Hlloc : l ∈ abstracts_local_vars rabs) by
+          now rewrite elem_of_abstracts_local_vars; eauto.
+        rewrite <- Hldom in Hlloc.
+        unfold ml'.
+        rewrite lookup_fmap, lookup_total_alt.
+        apply elem_of_dom in Hlloc as [v Hv].
+        rewrite Hv.
+        cbn.
+        destruct v as [r| |]; [|reflexivity..].
+        cbn.
+        rewrite (decide_False (mb !!! _)) by lia.
+        rewrite <- decide_not, (decide_ext _ (Pmap_map rrest_map r < lengthP unused_tys))
+          by lia.
+        replace (pos_sub_N _ _) with (Pmap_map rrest_map r) by lia.
+        f_equal.
+        symmetry.
+        move Hlimg at bottom.
+        specialize (Hlimg (rel r)).
+        tspecialize Hlimg by now apply elem_of_map_img; eauto.
+        assert (Hrabs : r ∈ abstracts_rel_vars tabs). 1:{
+          clear - Hlimg.
+          set_unfold.
+          rewrite !exists_pair in *.
+          setoid_rewrite elem_of_list_omap.
+          naive_solver.
+        }
+        apply Hrrest_inv_inv; [easy|].
+        rewrite Hldisj; [easy|].
+        subst mlran.
+        apply elem_of_map_img.
+        exists l.
+        rewrite lookup_omap, Hv.
+        reflexivity.
+Qed.
+
+
+
+(* TODO: Correctness of substitution!!! Then I'm honestly pretty close to done (I hope I swear plase don't make me regret writing this)
+
+  Using fill_tensorlist_rewrite, just need to figure out
+  typing requirements and how to induct and then I'm golden! I hope...
+  NB: I think the best way to approach doing _this_ is to set up
+  the lemma rephrasing semantics of fill_tensorlist_rewrite
+  (including switching from reasoning about substituted terms
+   to reasoning about semantics with precomposed term maps/contexts)
+
+  So, first lemma should be something like :
+    tl_total_semantics _* (fill_tensorlist_rewrite outer inner relmap locmap) =
+    [something like]
+    ∑ (outer sum shenanigans...),
+    tl_total_semantics [NOT THE SAME AS _*; modified using relmap / locmap; possibly want to unfold with the alternate semantics to permute the maps directly]
+    * (outer sum abstracts).
+  Then, correctness of [tl_tensor_equation] in terms of
+  extensionality of [tl_total_semantics] based on well-typed term maps,
+  and we can just do that rewrite
+*)
+
+
+
+
+
+
+
+
+
+
+
+
+
+
+
+
+
+
+
+
+
+
+
+
+
+
+
+
+
+
+
+
+
 
 
